src/coq/Trace.v
@@ -8,9 +8,13 @@
  *   3 of the License, or (at your option) any later version.                 *
  ---------------------------------------------------------------------------- *)
 
+Require Import ZArith Omega.
 Require Import  Vellvm.Classes Vellvm.Util.
 Require Import Program Classical.
 Require Import paco.
+Require Import Morphisms.
+Require Import Setoid.
+Require Import Relation_Definitions.
 
 Set Implicit Arguments.
 Set Contextual Implicit.
@@ -65,6 +69,18 @@ Definition idM E X (i: M E X) :=
 Lemma matchM : forall E X (i: M E X), i = idM i.
 Proof. destruct i; auto. Qed.
 
+
+(* Allow rewrite on both LHS and RHS *)
+Lemma matchM' : forall E X (i1 i2: M E X), i1 ≡ i2 <-> idM i1 ≡ idM i2.
+Proof.
+  split; intros.
+  - congruence.
+  - rewrite matchM.
+    rewrite @matchM with (i := i2).
+    auto.
+Qed.
+  
+
 (** [M E] forms a [Monad] *)
 (* N.b.: Possible variant: remove the Tau in the Ret case.  Not clear
    whether this is a global win (we have to then put some extra Taus
@@ -93,7 +109,7 @@ Definition mapM {E X Y} (f:X -> Y) (s: M E X) : M E Y :=
 Instance functor_M {E} : Functor (M E) := (@mapM E).
 Instance monad_M {E} : (@Monad (M E)) (@mapM E) := { mret X x := Ret x; mbind := @bindM E }.
 
-(* Properties of Traces ----------------------------------------------------- *)
+(* Properties of  ----------------------------------------------------- *)
 
 CoInductive equiv {E X} : M E X -> M E X -> Prop :=
 | equiv_Ret : forall x, equiv (Ret x) (Ret x)
@@ -102,7 +118,7 @@ CoInductive equiv {E X} : M E X -> M E X -> Prop :=
 | equiv_Err : forall s1 s2, equiv (Err s1) (Err s2)
 .
                              
-(* Properties of Traces ----------------------------------------------------- *)
+(* Properties of  ----------------------------------------------------- *)
 
 Module MonadVerif.
 (* Monad laws:
@@ -129,6 +145,7 @@ Inductive UnTau E X : M E X -> M E X -> Prop :=
 | OneTau : forall s t, UnTau s t -> UnTau (Tau s) t
 | NoTau : forall s, (forall t, ~(Tau t = s)) -> UnTau s s.
 
+
 CoInductive EquivUpToTau E X :
   M E X -> M E X -> Prop :=
 | EquivRet : forall x, EquivUpToTau (Ret x) (Ret x)
@@ -152,6 +169,88 @@ CoInductive EquivUpToTau E X :
 | EquivErr : forall s1 s2, EquivUpToTau (Err s1) (Err s2)
 .
 
+
+
+(* Tractic to force a Trace computation *)
+Ltac forcetrace :=
+  simpl;
+  match goal with
+  | [ |- ?X ≡ ?Y ] => rewrite matchM with (i := X);
+                    rewrite matchM with (i := Y);
+                    simpl; auto
+  | [H : _ |- _] => idtac H
+  | [ |- _ ] => idtac
+    end.
+
+
+Inductive EquivUpToTauGen E X (Rel: M E X -> M E X -> Prop) : M E X -> M E X -> Prop :=
+| _EquivRet : forall x, EquivUpToTauGen Rel (Ret x) (Ret x)
+| _EquivVis : forall Y (e : E Y) (k1 k2 : Y -> M E X)
+    (RELK: forall y,  Rel (k1 y) (k2 y)),
+    EquivUpToTauGen Rel (Vis e k1) (Vis e k2)
+(* Equality with spin is undecidable,
+   but one can coinductively generate a proof with this. *)
+| _EquivTau : forall s t (REL:  Rel s t),
+    EquivUpToTauGen Rel (Tau s) (Tau t)
+| _EquivTauLeft : forall s s' t (NOTAUT': forall t', ~(Tau t' = t))
+                    (UNTAUS: UnTau s s')
+                    (REL: Rel s' t),
+    EquivUpToTauGen Rel (Tau s) t
+| _EquivTauRight : forall s t t',
+    (forall s', ~(Tau s' = s)) ->
+    UnTau t t' ->
+    Rel s t' ->
+    EquivUpToTauGen Rel s (Tau t)
+| _EquivErr : forall s1 s2, EquivUpToTauGen Rel (Err s1) (Err s2)
+.
+
+
+(* Parametrized equiv up to tau relation *)
+Definition pEquivUpToTau E X mex1 mex2 :=
+  paco2 (@EquivUpToTauGen E X) bot2 mex1 mex2.
+Check (pEquivUpToTau).
+
+Hint Unfold pEquivUpToTau.
+Lemma pEquivUpToTauGen_monotone: forall E X,
+    monotone2 (@EquivUpToTauGen E X).
+Proof.
+  intros until X.
+  unfold monotone2.
+  intros.
+  induction IN.
+  - constructor.
+  - constructor.
+    intros.
+    apply LE.
+    apply RELK.
+  - constructor.
+    auto.
+  - eapply _EquivTauLeft; eauto.
+  - eapply _EquivTauRight; eauto.
+  - constructor.
+Qed.
+Hint Resolve pEquivUpToTauGen_monotone : paco.
+
+Lemma peutt_refl : forall E X (s : M E X),
+    pEquivUpToTau s s.
+Proof.
+  intros until X.
+  pcofix CIH.
+  intros; destruct s.
+  - pfold. constructor.
+  - apply paco2_fold.
+    constructor.
+    intros.
+    right.
+    apply CIH.
+
+    
+  - pfold. constructor.
+    right. auto.
+    
+  - pfold. constructor.
+Qed.
+
 Lemma eutt_refl : forall E X (s : M E X),
     EquivUpToTau s s.
 Proof.
@@ -173,6 +272,222 @@ Proof.
   - econstructor. assumption. eassumption. apply eutt_sym. assumption.
   - econstructor. assumption. eassumption. apply eutt_sym. assumption.
 Qed.
+
+Lemma peutt_sym : forall E X (s : M E X),
+    pEquivUpToTau s s.
+Proof.
+  intros until X.
+  pcofix CIH.
+  intros; destruct s.
+  - pfold. constructor.
+  - apply paco2_fold.
+    constructor.
+    intros.
+    right.
+    apply CIH.
+
+    
+  - pfold. constructor.
+    right. auto.
+    
+  - pfold. constructor.
+Qed.
+
+
+Fixpoint tauN {E X} (n: nat) (s': M E X): M E X :=
+  match n with
+  | 0 => s'
+  | S n' =>  Tau (tauN n' s')
+  end.
+
+Lemma tauN_destruct: forall {E X} (n: nat) (s': M E X),
+    tauN (n + 1) s' = Tau (tauN n s').
+Proof.
+  intros.
+  assert (N_PLUS_1: n + 1 = S n).
+  omega.
+  rewrite N_PLUS_1.
+  auto.
+Qed.
+
+
+Lemma tauN_untau:
+  forall E X
+    (n: nat)
+    (a: M E X),
+    (forall t: M E X, a <> Tau t) ->
+    UnTau (tauN n a) a.
+Proof.
+  intros until n.
+  induction n.
+  - intros. simpl.
+    constructor. auto.
+  - intros.
+    specialize (IHn a H).
+    replace (S n) with (n + 1)%nat.
+    rewrite tauN_destruct.
+    constructor. auto.
+    omega.
+Qed.
+
+
+Hint Resolve tauN_untau.
+    
+Lemma tauN_destruct_2:
+  forall {E X}
+    (n: nat)
+    (a: M E X),
+    tauN n (Tau a) = tauN (n + 1) a.
+Proof.
+  intros until n.
+  induction n.
+  - simpl. auto.
+  - simpl.
+    intros.
+    rewrite <- IHn.
+    auto.
+Qed.
+
+Lemma tauN_eutt: forall {E X}
+                   (n: nat)
+                   (a: M E X),
+    EquivUpToTau a (tauN n a).
+Proof.
+  intros until X.
+  cofix.
+
+  intros.
+
+
+  assert (NCASES: (n = 0 \/ n > 0)%nat).
+  omega.
+
+  destruct NCASES as [NZERO | NNONZERO].
+  - subst. apply eutt_refl.
+  - assert (N_AS_N': exists n', n = S n').
+    induction n.
+    omega.
+    eauto.
+
+    destruct N_AS_N' as [N' N'WITNESS].
+    subst.
+
+    replace (S N') with (N' + 1)%nat.
+    rewrite tauN_destruct.
+    Guarded.
+
+    destruct a;
+      try (eapply EquivTauRight; eauto; apply eutt_refl).
+
+    Guarded.
+    rewrite tauN_destruct_2.
+    Guarded.
+    constructor.
+    apply tauN_eutt.
+    Guarded.
+    omega.
+Qed.
+
+
+(* 
+Lemma tauN_peutt_left: forall {E X}
+                         (n: nat)
+                         (a: M E X),
+    pEquivUpToTau (tauN n a) a.
+Proof.
+  intros.
+  pcofix CIH.
+
+  assert (NCASES: (n = 0 \/ n > 0)%nat).
+  omega.
+
+  destruct NCASES as [NZERO | NNONZERO].
+  - rewrite NZERO in *. simpl in *.
+    apply eutt_refl.
+  - assert (N_AS_N': exists n', n = S n').
+    induction n.
+    omega.
+    eauto.
+    generalize dependent a.
+    intros.
+
+    destruct N_AS_N' as [N' N'WITNESS].
+    rewrite N'WITNESS in *.
+           
+
+    replace (S N') with (N' + 1)%nat; try omega.
+    rewrite tauN_destruct.
+    
+      
+    
+    destruct a; pfold.
+    eapply _EquivTauLeft.
+    eauto.
+    eauto.
+    pauto.
+    eapply eutt_refl.
+    pfold.
+
+    
+    Guarded.
+    rewrite tauN_destruct_2.
+    Guarded.
+    constructor.
+    apply tauN_eutt.
+    Guarded.
+    omega.
+Abort.
+*)
+
+
+(* Simple helpers for small applications of Tau *)
+Lemma tauN_eutt_1: forall {E X} (a: M E X),
+    EquivUpToTau a (Tau a).
+Proof.
+  intros.
+  replace (Tau a) with (tauN 1 a).
+  apply tauN_eutt.
+  auto.
+Qed.
+
+
+(* Simple helpers for small applications of Tau *)
+Lemma tauN_eutt_2: forall {E X} (a: M E X),
+    EquivUpToTau a (Tau (Tau a)).
+Proof.
+  intros.
+  replace (Tau (Tau a)) with (tauN 2 a).
+  apply tauN_eutt.
+  auto.
+Qed.
+    
+(* 
+Lemma tauN_destruct_2: forall {E X} (n: nat) (s': M E X),
+    tauN (S n) (Tau s') = tauN n s'.
+Proof.
+Qed.
+*)
+               
+
+(* Note that backward is not true, since this whole is lazy,
+you could have an INIFNITE stream of Tau (Tau (Tau (...)))) *)
+Lemma untau_count_layers:
+  forall E X (s t: M E X),
+    UnTau s t ->
+    exists (n: nat), s = tauN n t.
+Proof.
+  intros.
+  induction H.
+  - destruct IHUnTau as [n WITNESS].
+    exists (n + 1).
+    rewrite tauN_destruct.
+    rewrite WITNESS.
+    reflexivity.
+  - exists 0.
+    simpl.
+    reflexivity.
+Qed.
+  
 
 Lemma untau_notau : forall E X (s t : M E X), ~(UnTau s (Tau t)).
 Proof.
@@ -277,6 +592,20 @@ Proof.
     + constructor.
 Qed.
 
+
+Lemma eutt_untau_3: forall {E X} (t t': M E X),
+    UnTau t t' -> EquivUpToTau t t'.
+Proof.
+  intros.
+  assert (T_TAU: exists n, t = tauN n t').
+  apply untau_count_layers; auto.
+
+  destruct T_TAU as [N T_TAU].
+  rewrite T_TAU.
+  apply eutt_sym.
+  apply tauN_eutt.
+Qed.
+
 Lemma eutt_untau_trans : forall E X (s s' t : M E X),
     UnTau s s' -> EquivUpToTau s' t -> EquivUpToTau s t.
 Proof.
@@ -312,6 +641,37 @@ Proof.
   }
   assumption.
 Qed.
+
+
+
+(* bindM relationship with eutt*)
+Lemma eutt_bindM_through_tau: forall {E X Y} (x: M E X) (f: X -> M E Y),
+    EquivUpToTau (bindM (Tau x) f)  (bindM x f).
+Proof.
+  intros until Y.
+  cofix.
+
+  intros.
+  rewrite matchM.
+  simpl.
+
+  unfold bindM.
+
+
+  remember (((cofix go (s : M E X) : M E Y :=
+        match s with
+        | Ret x0 => Tau (f x0)
+        | @Vis _ _ Y e k => Vis e (fun y : Y => go (k y))
+        | Tau k => Tau (go k)
+        | Err s0 => Err (Event:=E) (X:=Y) s0
+        end) x)) as BIND.
+  apply eutt_sym.
+  apply tauN_eutt_1.
+Qed.
+
+    
+    
+
 
 Import Logic.ProofIrrelevance.
 
@@ -455,7 +815,656 @@ Proof.
   - econstructor.
 Qed.
 
+
+(** Register EUTT as an equivalence relation **)
+Add Parametric Relation (E: Type -> Type) (X: Type): (M E X) (@EquivUpToTau E X)
+    reflexivity proved by (@eutt_refl E X)
+    symmetry proved by (@eutt_sym E X)
+    transitivity proved by (@eutt_trans E X) as EUTT.
+
+
+(* Placed this here because i need transitivity of EUTT *)
+Lemma eutt_bindM_through_tauN: forall {E X Y} (n: nat) (x: M E X) (f: X -> M E Y),
+    EquivUpToTau (bindM (tauN n x) f)  (bindM x f).
+Proof.
+  intros until Y.
+  intros n.
+  induction n.
+  - intros.
+    simpl.
+    apply eutt_refl.
+
+  - intros.
+    replace (S n) with (n + 1).
+    rewrite tauN_destruct.
+
+    assert (ONE_STEP: EquivUpToTau
+                        (bindM (Tau (tauN n x)) f)
+                        (bindM (tauN n x) f)).
+    apply eutt_bindM_through_tau.
+
+    assert (N_STEPS: EquivUpToTau
+               (bindM (tauN n x) f)
+               (bindM x f)).
+    auto.
+
+    eapply eutt_trans; eauto.
+    omega.
+Qed.
+
+
+Lemma eutt_bindM_through_unTau: forall {E X Y}  (t t': M E X) (f: X -> M E Y),
+    UnTau t t' ->
+    EquivUpToTau (bindM t f)  (bindM t' f).
+Proof.
+  intros.
+  assert (T_TAU: exists n: nat, t = tauN n t').
+  apply untau_count_layers; auto.
+
+  destruct T_TAU as [n T_TAU].
+  subst.
+  apply eutt_bindM_through_tauN.
+Qed.
+
+(* This is not true, consider t' = Ret x, then it cannot be the
+RHS of an UnTau in the result since Ret x >>= f = (Tau (f x)))
+*)
+Lemma untau_bindM: forall {E X Y} (t t': M E X) (f: X -> M E Y),
+    (forall x: X, t' <> Ret x) -> 
+    UnTau t t' -> UnTau (bindM t f) (bindM t' f).
+Proof.
+  intros until f.
+  intros T'_NOT_RET.
+  intros UNTAU.
+  induction UNTAU.
+  - rewrite (@matchM) with (i := bindM (Tau s) f).
+    simpl.
+    unfold bindM in *.
+    apply OneTau.
+    apply IHUNTAU; auto.
+
+  - destruct s.
+    + specialize (T'_NOT_RET x).
+      contradiction.
+    + apply NoTau.
+      intros.
+      rewrite (@matchM) with (i := bindM (Vis e k) f).
+      simpl.
+      discriminate.
+    + specialize (H s).
+      contradiction.
+    + rewrite (@matchM) with (i := bindM (Err s) f).
+      simpl.
+      apply NoTau; auto.
+Qed.
+ 
+    
+  
+ 
+  
+
+Instance reflexive_eutt {E} X : Reflexive (@EquivUpToTau E X).
+Proof.
+  unfold Reflexive.
+  intros.
+  apply eutt_refl.
+Qed.
+
+
+Instance symmetric_eutt{E} X : Symmetric (@EquivUpToTau E X).
+Proof.
+  unfold Symmetric.
+  intros.
+  apply eutt_sym; auto.
+Qed.
+
+
+Instance transitive_eutt{E} X : Transitive (@EquivUpToTau E X).
+Proof.
+  unfold Transitive.
+  intros.
+  eapply eutt_trans; eauto.
+Qed.
+
+  
+
+Instance equivalence_eutt {E} X: Equivalence (@EquivUpToTau E X).
+Proof.
+  split.
+  apply reflexive_eutt.
+  apply symmetric_eutt.
+  apply transitive_eutt.
+Qed.
+
 Instance equiv_eutt {E} X : Equiv (M E X) := (@EquivUpToTau E X).
+
+
+Lemma tauN_eutt_upto_untau: forall {E X}
+                              (n: nat)
+                              (a b: M E X)
+                              (EQ: UnTau a b),
+    EquivUpToTau a (tauN n b).
+Proof.
+  intros.
+  assert (EQ_A_B: EquivUpToTau a b).
+  apply eutt_untau_3. auto.
+
+  assert (EQ_B_TAUN: EquivUpToTau b (tauN n b)).
+  apply tauN_eutt.
+  rewrite eutt_trans; eauto.
+  apply eutt_refl.
+Qed.
+
+
+(* Show theorems about bind being proper wrt equivalences *)
+Lemma bindM_Ret: forall (A B: Type) (E: Type -> Type ) (a: A) (f: A -> M E B),
+    bindM (Ret a) f ≡ f a.
+Proof.
+  intros.
+  rewrite (@matchM) with (i := bindM (_) _).
+  simpl.
+  symmetry.
+  apply tauN_eutt_1.
+  Guarded.
+Qed.
+
+
+
+
+Lemma bindM_proper_wrt_eutt:
+  forall {A B: Type} {E: Type -> Type} (a a': M E A) (f: A -> M E B),
+    a ≡ a' -> bindM a f ≡ bindM a' f.
+Proof.
+  intros A B.
+  cofix.
+
+  intros until f.
+  intros EQUIV.
+
+  destruct a.
+  - inversion EQUIV; subst; try reflexivity.
+    destruct t'.
+    ++ assert (LAYERS_IN_T: exists n, t = tauN n (Ret x0)).
+       apply untau_count_layers.
+       auto.
+       destruct LAYERS_IN_T as [n LAYERS_WITNESS].
+       rewrite LAYERS_WITNESS.
+       rewrite <- tauN_destruct.
+
+       assert (REMOVE_LAYERS: bindM (tauN (n + 1) (Ret x0)) f ≡
+                                    bindM (Ret x0) f).
+       apply eutt_bindM_through_tauN.
+       rewrite REMOVE_LAYERS.
+
+       assert (X_EQ_X0: x = x0).
+       inversion H1. auto.
+
+       rewrite X_EQ_X0.
+       reflexivity.
+    ++ inversion H1.
+    ++ assert (~ (UnTau t (Tau t'))).
+       apply untau_notau.
+       contradiction.
+    ++ inversion H1.
+       Guarded.
+       
+  -
+    inversion EQUIV; subst.
+     
+    ++ replace e with e1.
+       replace k with k0.
+       *** rewrite (@matchM) with (i := bindM (Vis e1 k0) f).
+           rewrite (@matchM) with (i := bindM (Vis e1 k2) f).
+           intros.
+           simpl.
+           constructor.
+           intros.
+           Guarded.
+           unfold bindM in bindM_proper_wrt_eutt.
+           apply bindM_proper_wrt_eutt with (f := f)
+                                            (a := (k0 y))
+                                            (a' := k2 y).
+           apply H3.
+           Guarded.
+
+       *** apply inj_pair2 with (P := fun Y => Y -> M E A).
+         assumption.
+
+       *** apply inj_pair2 with (P := fun Y => E Y).
+         assumption.
+
+    ++ inversion H1; subst.
+       *** 
+
+           
+           rewrite (@matchM) with (i := bindM (Vis e _) f).
+           rewrite (@matchM) with (i := bindM (Tau t ) f).
+           simpl.
+           eapply EquivTauRight with (t' := bindM (Vis e1 k2) f).
+           intros. discriminate.
+           Check (t).
+           Check (untau_bindM).
+           Check (Vis e1 k2).
+           
+
+           (* 
+            Lemma untau_bindM: forall {E X Y} (t t': M E X) (f: X -> M E Y),
+                (forall x: X, t' <> Ret x) -> 
+                UnTau t t' -> UnTau (bindM t f) (bindM t' f). *)
+           (* TODO: Understand why the variables got named
+           t0 and f0 *)
+           apply untau_bindM with
+               (t0 := t)
+               (t' := (Vis e1 k2))
+               (f0 := f); auto.
+           Guarded.
+           rewrite (@matchM) with (i := bindM (Vis e1 _) f).
+           simpl.
+           replace e1 with e.
+           
+           constructor.
+           Guarded.
+           intros.
+           Guarded.
+           apply bindM_proper_wrt_eutt with  (f:= f)
+                                             (a := k y)
+                                             (a' := k2 y).
+           replace k with k0.
+           apply H6.
+           Guarded.
+
+           apply inj_pair2 with (P := fun Y => Y -> M E A); auto.
+           apply inj_pair2 with (P := fun Y => E Y); auto.
+
+       
+       *** assert (CONTRA: ~ (UnTau t (Tau t0))).
+           apply untau_notau.
+           contradiction.
+
+
+  - Guarded.
+    inversion EQUIV.
+    ++ subst.
+       rewrite (@matchM) with (i := bindM (Tau a) f).
+       rewrite (@matchM) with (i := bindM (Tau t) f).
+       simpl.
+       constructor.
+
+       assert (A_EQUIV_T: a ≡ t).
+       auto.
+
+       apply bindM_proper_wrt_eutt with (a := a) (a':= t) (f := f); auto.
+       Guarded.
+       
+    ++ subst.
+       destruct s'.
+       *** inversion H2; subst.
+           assert (A_AS_TAU_RET_X: exists n, a = tauN n (Ret x)).
+           apply untau_count_layers; auto.
+           
+           destruct A_AS_TAU_RET_X as [N A_AS_TAU_RET_X].
+           rewrite A_AS_TAU_RET_X.
+           rewrite <- tauN_destruct.
+
+           assert (REMOVE_TAUN: bindM (tauN (N + 1) (Ret x)) f ≡ bindM (Ret x) f).
+           replace (N + 1)%nat with (S N).
+           apply eutt_bindM_through_tauN.
+           omega.
+
+           rewrite REMOVE_TAUN.
+           Guarded.
+
+           rewrite (@matchM) with (i := bindM (Ret _) _).
+           simpl.
+           reflexivity.
+           Guarded.
+
+           
+           rewrite (@matchM) with (i := bindM (Tau a) _).
+           rewrite (@matchM) with (i := bindM (Tau t) _).
+           simpl.
+           constructor.
+           apply bindM_proper_wrt_eutt with (f := f)
+                                            (a := a)
+                                            (a' := t).
+           Guarded.
+
+           assert (A_EQUIV_RET_X: a ≡ Ret x).
+           apply eutt_untau_3; auto.
+
+           assert (T_EQUIV_T': t ≡ t').
+           apply eutt_untau_3; auto.
+
+           rename H4 into RET_X_EQUIV_T'.
+
+           rewrite A_EQUIV_RET_X.
+           rewrite T_EQUIV_T'.
+           rewrite RET_X_EQUIV_T'.
+           reflexivity.
+           Guarded.
+
+       *** inversion H2; subst.
+           ---- 
+             rewrite (@matchM) with (i := bindM (Tau a) _).
+             rewrite (@matchM) with (i := bindM (Vis e1 k2) _).
+             simpl.
+             eapply EquivTauLeft with (s' := bindM (Vis e k) f).
+             intros. discriminate.
+             apply untau_bindM with (f0 := f)
+                                    (t := a)
+                                    (t' := (Vis e k)).
+             intros. discriminate.
+             assumption.
+
+             
+             rewrite (@matchM) with (i := bindM (Vis e k) _).
+             simpl.
+             Guarded.
+             replace e with e1.
+             replace k with k0.
+             constructor.
+             Guarded.
+             intros.
+             apply  bindM_proper_wrt_eutt with (f := f)
+                                               (a := k0 y)
+                                               (a' := k2 y).
+             apply H6.
+             Guarded.
+             apply inj_pair2 with (P := fun Y => Y -> M E A); auto.
+             apply inj_pair2 with (P := fun Y =>  E Y); auto.
+             
+             
+           ---- specialize (H0 t).
+                rename H0 into CONTRA.
+                contradiction.
+           
+         
+       *** assert (CONTRA: ~ (UnTau a (Tau s'))).
+           apply untau_notau.
+           contradiction.
+           Guarded.
+       *** inversion H2; subst.
+           rewrite (@matchM) with (i := bindM (Tau a) _).
+           rewrite (@matchM) with (i := bindM (Tau t) _).
+           simpl.
+           constructor.
+           apply bindM_proper_wrt_eutt with (f := f)
+                                            (a := a)
+                                            (a' := t).
+           Guarded.
+
+           assert (A_EQUIV_ERR: a ≡ Err s).
+           apply eutt_untau_3; auto.
+           rewrite A_EQUIV_ERR.
+           rewrite H2.
+           symmetry.
+           apply tauN_eutt_1.
+
+           rewrite (@matchM) with (i := bindM (Tau a) _).
+           rewrite (@matchM) with (i := bindM (Err _) _).
+           simpl.
+           apply EquivTauLeft with (s' := bindM (Err s) f).
+           Guarded.
+           intros; discriminate.
+           apply untau_bindM with
+               (f0 := f)
+               (t := a)
+               (t' := (Err s)).
+           intros. discriminate.
+           auto.
+           Guarded.
+           rewrite (@matchM) with (i := bindM (Err _) _).
+           simpl.
+           constructor.
+           
+           
+
+    ++ subst.
+       specialize (H a).
+       contradiction.
+
+  -  inversion EQUIV; subst.
+     
+     + rewrite (@matchM) with (i := bindM (Err s) f).
+       rewrite (@matchM) with (i := bindM (Tau _) f).
+       simpl.
+       apply EquivTauRight with (t' := bindM t' f).
+
+       **  intros; discriminate.
+       ** apply untau_bindM
+            with (f0 := f)
+                 (t0 := t)
+                 (t'0 := t').
+          inversion H1; subst; intros; discriminate.
+          auto.
+       ** replace (Err s) with (bindM (Err s) f).
+          apply bindM_proper_wrt_eutt; auto.
+          rewrite (@matchM) with (i := bindM (Err s) f).
+          auto.
+          Guarded.
+    
+       
+       
+     +  
+       rewrite (@matchM) with (i := bindM (Err s) f).
+       rewrite (@matchM) with (i := bindM (Err s2) f).
+       simpl.
+       constructor.
+       Guarded.
+Qed.
+
+Lemma bindM_rewrite_fn: 
+  forall {E: Type -> Type } {X Y: Type} (f g: X -> M E Y)
+  (EXT: forall (x: X), f x ≡ g x) (ex: M E X), bindM ex f ≡ bindM ex g.
+Proof.
+  intros until g.
+  intros EXT.
+  cofix.
+  destruct ex.
+  - rewrite @matchM  with (i := bindM (Ret x) f).
+    rewrite @matchM  with (i := bindM (Ret x) g).
+    simpl.
+    constructor.
+    apply EXT.
+    Guarded.
+
+  - rewrite @matchM  with (i := bindM (Vis e k) f).
+    rewrite @matchM  with (i := bindM (Vis e k) g).
+    simpl.
+    constructor.
+    intros.
+    apply bindM_rewrite_fn.
+    Guarded.
+
+  - rewrite @matchM  with (i := bindM (Tau ex) f).
+    rewrite @matchM  with (i := bindM (Tau ex) g).
+    simpl.
+    constructor.
+    apply bindM_rewrite_fn.
+    Guarded.
+
+  - rewrite @matchM  with (i := bindM (Err s) f).
+    rewrite @matchM  with (i := bindM (Err s) g).
+    simpl.
+    constructor.
+    Guarded.
+Qed.
+
+    
+    
+    
+Create HintDb eutt.
+Hint Resolve bindM_proper_wrt_eutt : eutt.
+
+
+Instance bindm_eutt_proper {E X Y}:
+  Proper ((@EquivUpToTau E X) ==> eq ==> (@EquivUpToTau E Y)) (@bindM E X Y).
+Proof.
+  intros.
+  intros MEX MEX'.
+  intros MEX_EQ_MEX'.
+
+  intros F G.
+  intros F_EQ_G.
+  subst.
+
+  apply bindM_proper_wrt_eutt.
+  assumption.
+Qed.
+
+Check (@bindM).
+Add Parametric Morphism (E: Type -> Type) (X Y : Type) : (@bindM E X Y) with
+      signature ((@EquivUpToTau E X) ==> eq ==> (@EquivUpToTau E Y)) as bind.
+Proof.
+  intros.
+  rewrite H.
+  reflexivity.
+Qed.
+
+
+
+Lemma eutt_coinduction_principle: forall E X (P: M E X -> M E X -> Prop)
+    (RET: forall t1 t2 x, P t1 t2 -> t1 = Ret x -> t2 = Ret x)
+    (VIS: forall {Y: Type }t1 t2 (e: E Y) (k1: Y -> M E X),
+        P t1 t2 ->
+        t1 = Vis e k1 ->
+        (exists (k2: Y -> M E X),
+            t2 = Vis e k2 /\
+            ((forall (y: Y), P (k1 y) (k2 y)))))
+    (TAU: forall t1 t2 t1',
+        P t1 t2 ->
+            t1 = Tau t1' /\
+            (exists t2', t2 = Tau t2' /\ P t1' t2'))
+    (ERR: forall t1 t2 s , t1 = Err (Event:=E) (X:=X) s ->
+                exists s', t2 = Err (Event:=E) (X:=X) s'),
+    (forall (t1 t2 : M E X), P t1 t2 -> EquivUpToTau t1 t2).
+Proof.
+  intros until P.
+  cofix.
+  intros until t2.
+  intros P_TRACES.
+  destruct t1.
+  + assert (T2_RET: t2 = Ret x).
+    eapply RET; eauto.
+    subst.
+    constructor.
+  + assert (T2_VIS: exists k2, t2 = Vis e k2 /\ (forall y:Y, P (k y) (k2 y))).
+    eapply VIS; eauto.
+    destruct T2_VIS as [k2' [T2_VIS KEQUIV]].
+    rewrite T2_VIS in *.
+    subst.
+    constructor.
+    Guarded.
+    intros.
+    apply eutt_coinduction_principle; auto.
+  + assert (T2TAU:  exists t2' : M E X, t2 = Tau t2' /\ P t1 t2').
+    eapply TAU; eauto.
+    destruct T2TAU as [t2' [T2TAu TEQUIV]].
+    subst.
+    constructor.
+    apply eutt_coinduction_principle; auto.
+  +
+    assert (T2ERR: exists s', t2 = Err s').
+    apply ERR with (t1 := (Err s)) (s := s); eauto.
+    
+    destruct T2ERR as [s' T2ERR].
+    subst.
+    constructor.
+Qed.
+
+(** Rewrite Rules **)
+
+
+Lemma bindM_Vis: forall {E: Type -> Type} {A B Y: Type} (e: E Y) (f: A -> M E B) (k: Y -> M E A),
+    bindM (Vis e k) f ≡ Vis e (fun y => bindM (k y) f).
+Proof.
+  intros until Y.
+  intros until k.
+  cofix.
+  intros.
+  rewrite @matchM with (i := (bindM (Vis e k) f)).
+  rewrite @matchM with (i := (Vis e (fun y => bindM (k y) f))).
+  simpl.
+
+  constructor.
+  intros.
+
+  destruct (k y) eqn:ky.
+  - rewrite @matchM. simpl.
+    rewrite @matchM with (i := ((cofix go (s : M E A) : M E B :=
+        match s with
+        | Ret x0 => Tau (f x0)
+        | @Vis _ _ Y0 e0 k0 => Vis e0 (fun y0 : Y0 => go (k0 y0))
+        | Tau k0 => Tau (go k0)
+        | Err s0 => Err (Event:=E) (X:=B) s0
+        end) (Ret x))). simpl. reflexivity. Guarded.
+
+  - rewrite @matchM with (i := ((cofix go (s : M E A) : M E B :=
+        match s with
+        | Ret x => Tau (f x)
+        | @Vis _ _ Y1 e1 k1 => Vis e1 (fun y0 : Y1 => go (k1 y0))
+        | Tau k1 => Tau (go k1)
+        | Err s0 => Err (Event:=E) (X:=B) s0
+        end) (Vis e0 k0))).
+    rewrite @matchM.
+    simpl.
+    constructor.
+    intros.
+    reflexivity.
+    Guarded.
+
+  - rewrite @matchM.
+    rewrite @matchM with (i :=
+                                  ((cofix go (s : M E A) : M E B :=
+                                      match s with
+                                      | Ret x => Tau (f x)
+                                      | @Vis _ _ Y0 e0 k0 => Vis e0 (fun y0 : Y0 => go (k0 y0))
+                                      | Tau k0 => Tau (go k0)
+                                      | Err s0 => Err (Event:=E) (X:=B) s0
+                                      end) (Tau m))).
+    simpl.
+    Guarded.
+    constructor. reflexivity.
+    Guarded.
+
+  - rewrite @matchM with (i :=
+                                  ((cofix go (s0 : M E A) : M E B :=
+                                      match s0 with
+                                      | Ret x => Tau (f x)
+                                      | @Vis _ _ Y0 e0 k0 => Vis e0 (fun y0 : Y0 => go (k0 y0))
+                                      | Tau k0 => Tau (go k0)
+                                      | Err s1 => Err (Event:=E) (X:=B) s1
+                                      end) (Err s))).
+    rewrite @matchM.
+    simpl.
+    reflexivity.
+    Guarded.
+Qed.
+
+
+
+
+
+(* 
+Instance eutt_proper_wrt_eutt_2 {X Y Z E } f:
+  Proper ((@EquivUpToTau E X) ==> (@EquivUpToTau E Y) ==> (@EquivUpToTau E Z)) f.
+Proof.
+  intros MEX MEX' MEX_EQ_MEX'.
+  intros MEY MEY' MEY_EQ_MEY'.
+Admitted.
+
+
+
+Instance eutt_proper_wrt_eutt_3 {X Y Z  A E } f:
+  Proper ((@EquivUpToTau E X)
+            ==> (@EquivUpToTau E Y)
+            ==> (@EquivUpToTau E Z) 
+            ==> (@EquivUpToTau E A)) f.
+Proof.
+Admitted.
+*)
+    
+
 
 (* SAZ: 
 Functoriality of (M E) probably holds only up to coinductively defined
@@ -466,14 +1475,54 @@ Instance M_functor_eutt_laws {E} : (@FunctorLaws (M E)) (@mapM E) (@equiv_eutt E
 Proof.
 Admitted.  
 
+(* (x >>= f) >> g ~= x >>= (fun x' => f x' >>= g ) *)
+Lemma bindM_assoc: forall {E: Type -> Type} {A B C: Type} (a: M E A) (f: A -> M E B)
+                     (g: B -> M E C),
+    (bindM (bindM a f) g) ≡ bindM  a (fun a' => bindM (f a') g).
+Admitted.
+
 Program Instance M_monad_eutt_laws {E} : (@MonadLaws (M E)) (@functor_M E) (@monad_M E) _ _ _.
 Next Obligation.
   Admitted.
 Next Obligation.
   Admitted.
 Next Obligation.
-  Admitted.
+Admitted.
+
+Check (M_monad_eutt_laws).
 
 
+
+Lemma remove_tau: forall {X: Type} {E: Type -> Type} (x: M E X), Tau x ≡ x.
+Proof.
+  intros.
+  repeat (rewrite <- tauN_eutt_1).
+  auto.
+Qed.
+
+
+Lemma bindM_Err: forall {X Y :Type} {E: Type -> Type} (e: String.string) (f: X -> M E Y),
+  bindM (Err e) f ≡ Err e.
+Proof.
+  intros.
+  rewrite @matchM with (i := (bindM _ _)).
+  auto.
+Qed.
+
+Create HintDb euttnormdb.
+Hint Rewrite (@bindM_assoc) : euttnormdb.
+Hint Rewrite (@bindM_Ret) : euttnormdb.
+Hint Rewrite (@bindM_Vis) : euttnormdb.
+Hint Rewrite (@remove_tau) : euttnormdb.
+Hint Rewrite (@bindM_Err) : euttnormdb.
+
+Ltac euttnorm := simpl; autorewrite with euttnormdb; simpl; auto.
+    
+
+Add Parametric Morphism (E: Type -> Type) (X : Type) : (@Tau E X) with
+      signature ((@EquivUpToTau E X) ==>(@EquivUpToTau E X)) as Tau.
+Proof.
+  intros.
+  constructor. auto.
+Qed.
 End MonadVerif.
-
