src/coq/MulAdd.v
@@ -1,0 +1,123 @@
+(* -------------------------------------------------------------------------- *
+ *                     Vellvm - the Verified LLVM project                     *
+ *                                                                            *
+ *     Copyright (c) 2017 Steve Zdancewic <stevez@cis.upenn.edu>              *
+ *                                                                            *
+ *   This file is distributed under the terms of the GNU General Public       *
+ *   License as published by the Free Software Foundation, either version     *
+ *   3 of the License, or (at your option) any later version.                 *
+ ---------------------------------------------------------------------------- *)
+
+Require Import ZArith List String Omega.
+Require Import Program.
+Require Import  Vellvm.Classes Vellvm.Util.
+Require Import Vellvm.LLVMAst.
+Require Import Vellvm.CFG.
+Require Import Vellvm.Pass.
+
+Import ListNotations.
+Open Scope Z_scope.
+Open Scope string_scope.
+
+Set Implicit Arguments.
+Set Contextual Implicit.
+
+Require Import Vellvm.Memory.
+
+Check (OP_IBinop).
+
+Definition two : exp := EXP_Integer 2.
+Definition three_HACK : exp := EXP_Integer 3.
+
+Definition is_exp_equal_ints (e e': exp): bool :=
+  match e with
+  | EXP_Integer x =>
+    match e' with
+    | EXP_Integer y => x =? y
+    | _ => false
+    end
+  |  _ => false
+  end.
+      
+Fixpoint rewrite_exp  (e:exp) : exp :=
+  match e with
+  | OP_IBinop (Add false false) p v1 v2 =>
+    match p with
+      | TYPE_I 64 => if is_exp_equal_ints v1 v2 
+               then OP_IBinop (Mul false false) (TYPE_I 64) v1 two
+                    else e
+      | _ => e
+    end
+  | _ => e
+  end.
+
+Definition rewrite_instr(i: instr): instr :=
+  match i with
+  | INSTR_Op e => INSTR_Op (rewrite_exp e)
+  | _ => i
+  end.
+
+
+(* 
+Record block : Set :=
+  mk_block
+    {
+      blk_id    : block_id;
+      blk_phis  : list (local_id * phi);
+      blk_code  : code;
+      blk_term  : instr_id * terminator;
+    }.
+*)
+
+Definition rewrite_block: block -> block := liftInstrPassToBlockPass rewrite_instr.
+
+
+(* 
+Record definition (FnBody:Set) :=
+  mk_definition
+  {
+    df_prototype   : declaration;
+    df_args        : list local_id;
+    df_instrs      : FnBody;
+  }.
+*)
+(*
+Definition rewrite_definition(d: definition (list block)) :=
+  mk_definition (list block)
+    (df_prototype d) 
+    (df_args d)
+    (map rewrite_block (df_instrs d)).
+*)
+
+(* 
+Record modul (FnBody:Set) : Set :=
+  mk_modul
+  {
+    m_name: option string;
+    m_target: option string;
+    m_datalayout: option string;
+    m_type_defs: list (ident * typ);
+    m_globals: list global;
+    m_declarations: list declaration;
+    m_definitions: list (definition FnBody);
+  }.
+*)
+(* 
+Definition rewrite_modul(m: modul (list block)): modul (list block) :=
+  {| m_name := m_name m;
+     m_target := m_target m;
+     m_datalayout := m_datalayout m;
+     m_type_defs := m_type_defs m;
+     m_globals := m_globals m;
+     m_declarations := m_declarations m;
+     m_definitions := map rewrite_definition (m_definitions m);
+  |}.
+*)
+                                                      
+Definition rewrite_cfg: cfg -> cfg := liftBlockPassToCFGPass rewrite_block.
+
+Definition rewrite_cfg_definition: definition cfg -> definition cfg :=
+  liftCFGPassToCFGDefinitionPass rewrite_cfg.
+
+Definition rewrite_mcfg: mcfg -> mcfg :=
+  liftCFGDefinitionPassToMCFGPass rewrite_cfg_definition.
