src/coq/MulAddProof.v
@@ -1,0 +1,524 @@
+(* -------------------------------------------------------------------------- *
+ *                     Vellvm - the Verified LLVM project                     *
+ *                                                                            *
+ *     Copyright (c) 2017 Steve Zdancewic <stevez@cis.upenn.edu>              *
+ *                                                                            *
+ *   This file is distributed under the terms of the GNU General Public       *
+ *   License as published by the Free Software Foundation, either version     *
+ *   3 of the License, or (at your option) any later version.                 *
+ ---------------------------------------------------------------------------- *)
+
+
+Require Import ZArith List String Omega.
+Require Import Vellvm.AstLib Vellvm.LLVMAst.
+Require Import Vellvm.Classes.
+Require Import Vellvm.Util.
+Require Import Vellvm.MulAdd.
+Require Import Vellvm.CFG.
+Require Import Vellvm.LLVMIO.
+Require Import Vellvm.DynamicValues.
+Require Import Vellvm.StepSemantics.
+Require Import  Vellvm.Classes Vellvm.Util.
+Require Import Vellvm.LLVMAst.
+Require Import Vellvm.TypeUtil.
+Require Import Vellvm.Trace.
+Require Import Setoid.
+Require Import Coq.Setoids.Setoid.
+Require Import SetoidClass.
+Require Import Coq.Classes.RelationClasses.
+Require Import Coq.Classes.Equivalence.
+Require Import Vellvm.Pass.
+Require Import FunctionalExtensionality.
+Require Import Eqdep_dec.
+Require Import Program Classical.
+
+
+
+Open Scope Z_scope.
+Open Scope string_scope.
+
+
+Module MULADDPROOF (A:MemoryAddress.ADDRESS) (LLVMIO:LLVM_INTERACTIONS(A)).
+
+
+(* 
+Module SS := StepSemantics A LLVMIO.
+Import SS.
+*)
+
+Import LLVMIO.
+Import Trace.MonadVerif.
+
+Module PT := PASSTHEOREMS A LLVMIO.
+Import PT.
+
+Import PT.SS.
+
+(* Since
+1. Trace X := M IO X
+2. M is a free monad-style construction
+3. IO is a functor,
+
+M should lift the IO instance of function into a monad instance of (M IO).
+
+However, Coq typeclass syntax is.. difficult to someone who's never used it,
+so I'm going to Admit the monad laws for Trace (which will hold, asuming the M construction
+is correct)
+ *)
+
+
+Check (@bindM).
+Check (@mbind).
+
+(* Clearly, I'm able to use monads in the abstract. I'm just not able to convince coq that
+Trace is actually a Monad, even though
+ Definition Trace X := M IO X. 
+*)
+Example bind_of_ret: 
+  (mbind (F := M IO)) (mret (DVALUE_I64 (Int64.repr 2)))  (fun v => mret v)  ≡ mret (DVALUE_I64 (Int64.repr 2)).
+Proof.
+  apply mret_mbind.
+Qed.
+
+
+Lemma  eval_type_I64: forall (cfg: mcfg),
+    eval_typ cfg (TYPE_I 64) = DTYPE_I 64.
+Proof.
+  intros.
+  unfold eval_typ.
+  rewrite normalize_type_equation.
+  auto.
+Qed.
+
+Lemma eval_typ_rewrite_mcfg: forall (mcfg: mcfg) (t: typ),
+    eval_typ (rewrite_mcfg mcfg) t = eval_typ mcfg t.
+Proof.
+  intros.
+  repeat (unfold eval_typ).
+  repeat (rewrite normalize_type_equation).
+
+  destruct t; auto.
+Qed.
+
+Lemma transform_correct:
+  forall (i: Z),
+ (Int64.mul (Int64.repr i) (Int64.repr 2))
+  = (Int64.add (Int64.repr i) (Int64.repr i)).
+Proof.
+  intros.
+  unfold Int64.mul.
+  unfold Int64.add.
+  auto with ints.
+
+  assert (UNSIGNED_REPR_2: Int64.unsigned (Int64.repr 2) = 2).
+  rewrite Int64.unsigned_repr; auto with ints.
+  unfold Int64.max_unsigned. unfold Int64.modulus.
+  simpl. omega.
+
+  rewrite UNSIGNED_REPR_2.
+
+  assert (MUL2: forall x: Z, x * 2 = x + x).
+  intros. omega.
+
+  specialize (MUL2 (Int64.unsigned (Int64.repr i))).
+  rewrite MUL2.
+
+  reflexivity.
+Qed.
+
+
+Lemma is_exp_equal_ints_inv: forall (o1 o2: exp),
+    is_exp_equal_ints o1 o2 = true -> o1 = o2 /\
+                                     exists (x: int),  o1 = (EXP_Integer x) .
+Proof.
+  intros.
+  destruct o1; inversion H; destruct o2; inversion H; auto.
+  rewrite Z.eqb_eq in H1.
+  subst.
+  split; auto.
+  exists x0. auto.
+Qed.
+
+    
+      
+        
+
+
+Lemma map_monad_trace_cons: forall {A B}
+                        (f: A -> Trace  B)
+                        (x: A)
+                        (xs: list A),
+    map_monad f (x :: xs) ≡
+    'mx <- f x;
+    'mxs <- map_monad f xs;
+    mret (mx ::mxs).
+Proof.
+  intros.
+  simpl.
+  reflexivity.
+Qed.
+    
+  
+  
+
+
+
+Ltac unfold_fail :=  simpl; unfold failwith; unfold raise; unfold exn_trace; eauto.
+
+Lemma eval_exp_is_ret_or_err:
+  forall (expr: exp)
+    (MCFG: mcfg)
+    (ge: genv)
+    (e: env)
+    (top: option dtyp),
+    (exists x, eval_exp MCFG ge e top expr ≡ Ret x) \/
+    (exists err, eval_exp MCFG ge e top expr ≡ Err err).
+Proof.
+  intros expr.
+  induction expr; intros; simpl;
+    try (destruct top; try unfold_fail;
+         destruct d; try unfold_fail).
+  - destruct (lookup_id ge e id); eauto;
+      simpl; unfold raise. unfold exn_trace. eauto.
+    eauto.
+  - destruct (coerce_integer_to_int sz x); eauto.
+    (* ERROR, EAUTO DOES NOT WORK OVER EQUIVALENCE RELATIONS! *)
+    right. unfold_fail.
+    simpl.
+    unfold raise, exn_trace. eauto.
+    
+  - destruct b; eauto.
+  - (* Where is the induction principle? *)
+    simpl.
+    induction fields.
+    + simpl.
+      left.
+      exists (DVALUE_Struct []).
+      rewrite bindM_Ret.
+      auto.
+    + destruct IHfields.
+      * destruct H as [X XWITNESS].
+        simpl in *.
+        left.
+        exists (DVALUE_Struct [X]).
+        destruct a.
+        simpl.
+        admit.
+      * admit.
+                
+    
+  - admit.
+  - admit.
+  - admit .
+  - edestruct IHexpr1.
+    admit.
+Admitted.
+    
+  
+
+(* OP_IBinop (Add nuw_disabled nsw_disabled) (TYPE_I 64) v1 v2 *)
+Lemma eval_exp_equal: forall (mcfg : mcfg)
+                        (ge: genv)
+                        (e: env)
+                        (top: option dtyp)
+                        (o: exp),
+    eval_exp (rewrite_mcfg mcfg) ge e top (rewrite_exp o) ≡
+    eval_exp mcfg ge e top o.
+Proof.
+  intros.
+  induction o; simpl; try (apply MonadVerif.eutt_refl);
+  destruct iop; simpl; try (apply MonadVerif.eutt_refl);
+  destruct t; simpl; try (apply MonadVerif.eutt_refl);
+  destruct nuw; simpl; try (apply MonadVerif.eutt_refl);
+  destruct nsw; simpl; try (apply MonadVerif.eutt_refl);
+  destruct sz; simpl; try (apply MonadVerif.eutt_refl);
+  destruct p; simpl; try (apply MonadVerif.eutt_refl);
+  destruct p; simpl; try (apply MonadVerif.eutt_refl);
+  destruct p; simpl; try (apply MonadVerif.eutt_refl);
+  destruct p; simpl; try (apply MonadVerif.eutt_refl);
+  destruct p; simpl; try (apply MonadVerif.eutt_refl);
+  destruct p; simpl; try (apply MonadVerif.eutt_refl).
+  destruct p; simpl; try (apply MonadVerif.eutt_refl).
+  remember (is_exp_equal_ints o1 o2) as ISEQ.
+
+  assert (ISEQ_CASES: {ISEQ = true} + {ISEQ <> true}).
+  decide equality.
+
+  destruct ISEQ_CASES as [ISEQ_TRUE | ISEQ_FALSE]; subst.
+
+  --  rewrite ISEQ_TRUE.
+
+      assert (EXPLOIT_EQ_INT: o1 = o2 /\ exists x, o1 = EXP_Integer x).
+      apply is_exp_equal_ints_inv; auto.
+
+      
+      destruct EXPLOIT_EQ_INT as [EQ_INT  INT_DESCRIPTION].
+      subst.
+      destruct INT_DESCRIPTION as [i O2_AS_INT].
+      subst.
+      simpl.
+      
+      rewrite eval_typ_rewrite_mcfg.
+      repeat (rewrite eval_type_I64).
+      simpl.
+
+      repeat (rewrite bindM_Ret).
+      simpl.
+      rewrite transform_correct.
+      auto.
+
+
+
+  -- rewrite Bool.not_true_iff_false in ISEQ_FALSE.
+     rewrite ISEQ_FALSE.
+     simpl.
+     apply eutt_refl.
+Qed.
+
+
+Lemma lifted_instruction_pass_preserves_block_term_id:
+  forall (b : LLVMAst.block),
+  blk_term_id (liftInstrPassToBlockPass rewrite_instr b) =
+  blk_term_id b.
+Proof.
+  auto.
+Qed.
+
+Hint Resolve (lifted_instruction_pass_preserves_block_term_id).
+Hint Rewrite (lifted_instruction_pass_preserves_block_term_id).
+  
+
+
+Lemma bindm_eval_exp_equal: forall CFG g e op fn bk a s id,
+  bindM
+    (eval_exp (liftCFGDefinitionPassToMCFGPass rewrite_cfg_definition CFG) g e
+       None (rewrite_exp op))
+    (fun dv : dvalue =>
+     cont (g, {| fn := fn; bk := bk; pt := a |}, add_env id dv e, s))
+  ≡ bindM (eval_exp CFG g e None op)
+      (fun dv : dvalue =>
+         cont (g, {| fn := fn; bk := bk; pt := a |}, add_env id dv e, s)).
+Proof.
+  intros until CFG.
+  cofix.
+
+  intros.
+
+  (* I do it this way because somehow, applying `symmetry` breaks
+  the guardedness condition. TODO: Figure this out, the correct way *)
+  rewrite (@Trace.matchM) with (i := bindM (eval_exp CFG g e None op)
+                                           (fun dv : dvalue =>
+                                              cont (g, {| fn := fn; bk := bk; pt := a |}, add_env id dv e, s))).
+  rewrite Trace.matchM.
+
+  simpl.
+
+  assert (EVAL_EXP_EQ: eval_exp
+            (liftCFGDefinitionPassToMCFGPass rewrite_cfg_definition CFG) g e
+            None (rewrite_exp op) ≡
+            eval_exp CFG g e None op).
+  auto.
+
+  remember (eval_exp CFG g e None (rewrite_exp op)) as EVAL_EXP_ORIG.
+
+  destruct (EVAL_EXP_ORIG); simpl; auto.
+Abort.
+
+  
+  
+Lemma muladd_step: forall (CFG: mcfg) (s: state),
+    step (rewrite_mcfg CFG) s ≡ step CFG s.
+Proof.
+  intros.
+  unfold step.
+  
+  destruct s.
+  
+  destruct p.
+  destruct p.
+
+  
+  unfold fetch.
+  destruct p.
+
+  unfold rewrite_mcfg.
+  rewrite find_function_lifted_definition_pass.
+  simpl.
+
+  remember (find_function CFG fn) as CURFN.
+  destruct CURFN; simpl; try reflexivity.
+
+  rewrite find_block.
+
+  remember (CFG.find_block (blks (df_instrs d)) bk) as CURBLOCK.
+  destruct CURBLOCK; simpl; try reflexivity.
+
+
+  unfold rewrite_block.
+  rewrite InstrPassPreservesBlockToCmd.
+  simpl.
+
+  remember (block_to_cmd b pt) as CURCMD.
+  destruct CURCMD; auto.
+  destruct p.
+  simpl.
+  
+
+  assert (FNEQ:
+            find_function
+              (liftCFGDefinitionPassToMCFGPass rewrite_cfg_definition CFG) =
+            fun fnid => option_map rewrite_cfg_definition (find_function CFG fnid)).
+  extensionality fid_ext.
+  apply find_function_lifted_definition_pass.
+  auto.
+
+  assert (EVAL_TYP_EQ:
+            (eval_typ
+               (liftCFGDefinitionPassToMCFGPass rewrite_cfg_definition CFG) =
+             eval_typ CFG)).
+  unfold eval_typ.
+  extensionality typ_ext.
+  apply preserves_types_implies_preserves_eval_typ.
+  unfold preserves_types.
+  auto.
+
+  assert (EVAL_EXP_EQ:
+            eval_exp
+              ((liftCFGDefinitionPassToMCFGPass rewrite_cfg_definition) CFG) =
+            eval_exp CFG).
+  extensionality g_ext.
+  extensionality e_ext.
+  extensionality t_ext.
+  extensionality expr_ext.
+  apply preserves_types_implies_preserves_eval_expr.
+  unfold preserves_types.
+  auto.
+
+  assert (EVAL_JUMP_EQ:
+            jump (liftCFGDefinitionPassToMCFGPass rewrite_cfg_definition CFG) =
+            jump CFG).
+  intros.
+  
+  unfold jump.
+  extensionality fid_ext.
+  extensionality bid_src_ext.
+  extensionality bid_tgt_ext.
+  extensionality g_ext.
+  extensionality e_ext.
+  extensionality k_ext.
+  apply eq_jump; auto.
+  unfold preserves_types; auto.
+  apply lifted_instr_pass_to_MCFG_pass_preserves_block_entry.
+  
+
+
+  assert (EVAL_FIND_FUNCTION_EQ:
+            find_function_entry
+              (liftCFGDefinitionPassToMCFGPass rewrite_cfg_definition CFG)
+            = find_function_entry CFG).
+  intros.
+  extensionality fid.
+  apply lifted_instr_pass_preserves_function_entry.
+
+  (* 
+  assert (EVAL_OP_EQ:
+          eval_op
+             (liftCFGDefinitionPassToMCFGPass rewrite_cfg_definition CFG) ≡
+          eval_op CFG).
+  unfold eval_op.
+  extensionality g_ext.
+  extensionality e_ext.
+  extensionality o_ext.
+  apply eval_exp_equal.
+  *)
+
+  destruct c; auto; simpl.
+  
+  - simpl.
+    repeat (rewrite EVAL_TYP_EQ).
+    repeat (rewrite EVAL_EXP_EQ).
+    repeat (rewrite FNEQ).
+    repeat (rewrite EVAL_JUMP_EQ).
+    repeat (rewrite EVAL_FIND_FUNCTION_EQ).
+
+    destruct (find_function CFG fn); auto; simpl.
+    rewrite find_block; auto.
+    destruct (CFG.find_block (blks (df_instrs d0)) bk); auto; simpl.
+
+    unfold rewrite_block; auto.
+    rewrite (InstrPassPreservesBlockToCmd).
+    destruct (block_to_cmd b0 pt); auto; simpl.
+
+    
+    induction p; simpl; auto.
+    induction a; simpl; auto.
+    ++ induction b1; simpl; auto.
+       induction pt; simpl; auto.
+       *** induction i; simpl; auto.
+           unfold eval_op.
+
+           assert (CUR_REWRITE: eval_exp
+                     (liftCFGDefinitionPassToMCFGPass rewrite_cfg_definition CFG)
+                     g
+                     e
+                     None
+                     (rewrite_exp op) ≡ eval_exp CFG g e None op).
+           rewrite eval_exp_equal.
+           reflexivity.
+           (* Why can't I rewrite here? Because it's inside a cofix? *)
+           admit.
+
+       *** induction i; simpl; auto.
+    ++ induction b1; simpl; auto.
+       induction pt; simpl; auto.
+       *** induction i; simpl; auto.
+           unfold eval_op.
+           (* Again, why can't I rewrite? *)
+           admit.
+       *** induction i; simpl; auto.
+       
+
+      
+  - simpl.
+    repeat (rewrite EVAL_TYP_EQ).
+    repeat (rewrite EVAL_EXP_EQ).
+    repeat (rewrite FNEQ).
+    repeat (rewrite EVAL_JUMP_EQ).
+    reflexivity.
+
+  -  auto.
+  -  auto. 
+
+Admitted.
+
+(* 
+CoFixpoint step_sem (r:result) : Trace dvalue :=
+  match r with
+  | Done v => mret v
+  | Step s => 'x <- step s ; step_sem x
+  end.
+ *)
+
+  
+
+          
+ 
+(* How do I force one step of step_sem? *)
+Lemma step_sem_unfold_once: forall (CFG: mcfg) (s: state),
+    step_sem CFG (Step s) ≡ ('x <- (step CFG s); (step_sem CFG x)).
+Proof.
+  intros.
+  unfold step_sem.
+  rewrite Trace.matchM.
+  simpl.
+
+  destruct (step CFG s).
+  - rewrite bindM_Ret.
+Abort.
+
+Lemma muladd_step_sem : forall (CFG:mcfg) (r:result),
+    (step_sem (rewrite_mcfg CFG) r) ≡ (step_sem CFG r).
+Proof.
+Abort.
+  
+End MULADDPROOF.
