src/coq/Pass.v
@@ -1,0 +1,640 @@
+(* Infrastructure for writing passes and lemmas about passes *)
+Require Import ZArith List String Omega.
+Require Import Program.
+Require Import  Vellvm.Classes Vellvm.Util.
+Require Import Vellvm.LLVMAst.
+Require Import Vellvm.CFG.
+Require Import ZArith List String Omega.
+Require Import Vellvm.AstLib Vellvm.LLVMAst.
+Require Import Vellvm.Classes.
+Require Import Vellvm.Util.
+Require Import Vellvm.CFG.
+Require Import Vellvm.LLVMIO.
+Require Import Vellvm.DynamicValues.
+Require Import Vellvm.StepSemantics.
+Require Import  Vellvm.Classes Vellvm.Util.
+Require Import Vellvm.LLVMAst.
+Require Import Vellvm.TypeUtil.
+Require Import Vellvm.Trace.
+Require Import Setoid Morphisms.
+Require Import Coq.Setoids.Setoid.
+Require Import SetoidClass.
+Require Import Coq.Classes.RelationClasses.
+Require Import Coq.Classes.Equivalence.
+Require FunctionalExtensionality.
+
+Import ListNotations.
+Open Scope Z_scope.
+Open Scope string_scope.
+
+Set Implicit Arguments.
+Set Contextual Implicit.
+
+Require Import Vellvm.Memory.
+
+Definition Pass (A: Type) := A -> A.
+
+Definition InstrPass := Pass instr.
+Definition CodePass := Pass code.
+Definition BlockPass := Pass block.
+Definition CFGPass := Pass cfg.
+Definition CFGDefinitionPass := Pass (definition cfg).
+Definition MCFGPass := Pass mcfg.
+
+(* We can create fancy typeclass based machinery to lift passes to
+their correct embedding, similar to the way in which effect handlers
+get resolved (At least, I think this is possible), but let's not, for now *)
+
+(* --- Lemmas --- *)
+
+Definition liftInstrPassToIdInstrPass (pass: InstrPass):
+  Pass (instr_id * instr) :=
+  fun x => (fst x, pass (snd x)).
+  
+
+
+
+(* NOTE: Define it this way so that we don't modify the first instruction.
+If we modify the first instruction, this will fuck up jumps *)
+(* NOTE: My understading was slightly flawed. It uses *ID* of the
+first instruction. Which is still crazy, because me removing the first
+instruction will cause `jump` behaviour to change *)
+Definition liftInstrPassToBlockPass (pass: InstrPass): BlockPass :=
+  fun (b: block) =>
+    mk_block (blk_id b)
+                (blk_phis b)
+                (List.map (liftInstrPassToIdInstrPass pass) (blk_code b))
+                (blk_term b).
+
+  
+
+Definition liftBlockPassToCFGPass (pass: BlockPass): CFGPass:=
+  fun (c: cfg) =>
+    {|
+      init := init c;
+      blks := map pass (blks c);
+      args := args c;
+    |}.
+
+Definition liftCFGPassToCFGDefinitionPass (pass: CFGPass): CFGDefinitionPass :=
+  fun (d: definition cfg) =>
+     mk_definition cfg
+                   (df_prototype d) 
+                   (df_args d)
+                   (pass (df_instrs d)).
+
+
+Definition liftCFGDefinitionPassToMCFGPass
+           (pass: CFGDefinitionPass): MCFGPass :=
+  fun (m: mcfg) =>
+    {| m_name := m_name m;
+       m_target:= m_target m;
+       m_datalayout := m_datalayout m;
+       m_type_defs := m_type_defs m;
+       m_globals := m_globals m;
+       m_declarations := m_declarations m;
+       m_definitions := map pass (m_definitions m);
+    |}.
+
+
+
+
+Open Scope Z_scope.
+Open Scope string_scope.
+
+
+Module PASSTHEOREMS (A:MemoryAddress.ADDRESS) (LLVMIO:LLVM_INTERACTIONS(A)).
+  (* Need this to simplify proofs, otherwise I need to painfully destruct
+  execution chains. *)
+Import FunctionalExtensionality.
+
+
+Module SS := StepSemantics A LLVMIO.
+Import SS.
+Import LLVMIO.
+
+(* Since
+1. Trace X := M IO X
+2. M is a free monad-style construction
+3. IO is a functor,
+
+M should lift the IO instance of function into a monad instance of (M IO).
+
+However, Coq typeclass syntax is.. difficult to someone who's never used it,
+so I'm going to Admit the monad laws for Trace (which will hold, asuming the M construction
+is correct)
+ *)
+
+Lemma bindM_Ret: forall (A B: Type) (a: A) (f: A -> Trace B),
+    bindM (Ret a) f ≡  f a.
+Proof.
+Admitted.
+
+Check (@bindM).
+Check (@mbind).
+
+(* Clearly, I'm able to use monads in the abstract. I'm just not able to convince coq that
+Trace is actually a Monad, even though
+ Definition Trace X := M IO X. 
+*)
+Example bind_of_ret: 
+  (mbind (F := M IO)) (mret (DVALUE_I64 (Int64.repr 2)))  (fun v => mret v)  ≡  mret (DVALUE_I64 (Int64.repr 2)).
+Proof.
+  apply mret_mbind.
+Qed.
+
+Hint Resolve bind_of_ret.
+Hint Rewrite -> bind_of_ret.
+
+Lemma  eval_type_I64: forall (cfg: mcfg),
+    eval_typ cfg (TYPE_I 64) = DTYPE_I 64.
+Proof.
+  intros.
+  unfold eval_typ.
+  rewrite normalize_type_equation.
+  auto.
+Qed.
+
+
+Hint Resolve eval_type_I64.
+
+Definition preserves_types (p: MCFGPass): Prop :=
+  forall (CFG: mcfg), m_type_defs (p CFG) = m_type_defs CFG.
+
+Definition preserves_eval_typ (p: MCFGPass) (MCFG: mcfg) (t: typ): Prop :=
+  eval_typ (p MCFG) t = eval_typ MCFG t.
+
+Lemma preserves_types_implies_preserves_eval_typ:
+  forall (p: MCFGPass) (CFG: mcfg) (t: typ),
+    preserves_types p ->
+    eval_typ (p CFG) t = eval_typ CFG t.
+Proof.
+  intros.
+  repeat (unfold eval_typ).
+
+  unfold preserves_types in H.
+  rewrite H.
+  repeat (rewrite normalize_type_equation).
+  destruct t; auto.
+Qed.
+
+Hint Resolve preserves_types_implies_preserves_eval_typ.
+
+Definition preserves_ident_definition (g: CFGDefinitionPass): Prop :=
+  forall (fn: definition cfg), ident_of (g fn) = ident_of fn.
+
+Hint Unfold preserves_ident_definition.
+
+Lemma lifted_cfg_pass_preserves_ident_definition: forall (pass: CFGPass),
+    preserves_ident_definition (liftCFGPassToCFGDefinitionPass pass).
+Proof.
+  intros.
+  auto.
+Qed.
+
+Hint Resolve lifted_cfg_pass_preserves_ident_definition.
+
+Lemma preserves_ident_definition_commutes_with_find_defn:
+  forall (fnid: function_id)
+    (g: CFGDefinitionPass),
+    preserves_ident_definition g ->
+    agress_on_filter (find_defn fnid) g.
+Proof.
+  intros until g.
+  intros PRESERVES_IDENT.
+  
+  unfold agress_on_filter.
+  intros.
+  split.
+
+  - intros.
+    unfold find_defn in *.
+    destruct (ident_of a == ID_Global fnid); try discriminate.
+    inversion H. subst.
+    exists (g b).
+
+    assert (IDENT_PRESERVED: ident_of (g b) = ID_Global fnid).
+    unfold preserves_ident_definition in PRESERVES_IDENT.
+    specialize (PRESERVES_IDENT b).
+    rewrite PRESERVES_IDENT.
+    rewrite e.
+    auto.
+
+
+    rewrite IDENT_PRESERVED.
+    destruct (ID_Global fnid == ID_Global fnid); auto; congruence.
+
+  - intros.
+    unfold preserves_ident_definition in PRESERVES_IDENT.
+    unfold find_defn in *.
+    destruct (ident_of a == ID_Global fnid); try discriminate.
+    assert (IDENT_GA: ident_of (g a) = ident_of a).
+    auto.
+
+    rewrite IDENT_GA.
+    destruct (ident_of a == ID_Global fnid); try contradiction; auto.
+Qed.
+Hint Resolve preserves_ident_definition_commutes_with_find_defn.
+   
+
+
+
+Lemma find_definition_some: forall (CFG: mcfg)
+                                 (fnid: function_id)
+                                (oldfn: definition cfg)
+                                (g: CFGDefinitionPass),
+
+  preserves_ident_definition g ->
+  find_function CFG fnid = Some oldfn ->
+  find_map (find_defn fnid) (map g (m_definitions CFG)) =
+  Some (g oldfn).
+Proof.
+  intros until g.
+  intros PRESERVES_IDENT FINDOLD.
+  assert (FIND_ON_MAP: exists old_old_fn, Some oldfn = (find_defn fnid old_old_fn) /\
+                        find_map (find_defn fnid) (map g (m_definitions CFG)) = (find_defn fnid (g old_old_fn))).
+  apply find_map_mapped_some_1; try assumption.
+  auto.
+
+  destruct FIND_ON_MAP as [OLD_OLD_FN [OLD_FN_AS_OLD_OLD_FN FIND_WITNESS]].
+  unfold find_defn in OLD_FN_AS_OLD_OLD_FN.
+  destruct (ident_of OLD_OLD_FN == ID_Global fnid); try discriminate.
+  inversion OLD_FN_AS_OLD_OLD_FN.
+  subst.
+
+  rewrite FIND_WITNESS.
+  unfold find_defn.
+
+  assert (ID_G_OLD_OLD_FN: ident_of (g OLD_OLD_FN) = ID_Global fnid).
+  unfold preserves_ident_definition in PRESERVES_IDENT.
+  rewrite <- e.
+  apply PRESERVES_IDENT.
+
+  rewrite ID_G_OLD_OLD_FN.
+  destruct (ID_Global fnid == ID_Global fnid); auto; try congruence.
+Qed.
+Hint Resolve find_definition_some.
+
+Lemma find_function_some: forall
+    (CFG: mcfg)
+    (fnid: function_id)
+    (oldfn: definition cfg)
+    (g: CFGDefinitionPass)
+    (PRESERVES_DEFN_IDENT: preserves_ident_definition g),
+    find_function CFG fnid = Some oldfn ->
+    find_function ((liftCFGDefinitionPassToMCFGPass g) CFG) fnid = Some (g oldfn).
+Proof.
+  intros.
+  unfold find_function in *.
+  simpl.
+  apply find_definition_some; auto.
+Qed.
+
+
+Hint Resolve find_function_some.
+
+Lemma find_function_none:
+  forall (CFG: mcfg)
+    (fnid: function_id)
+    (g: CFGDefinitionPass)
+    (PRESERVES_DEFN_IDENT: preserves_ident_definition g), 
+    find_function CFG fnid = None ->
+    find_function ((liftCFGDefinitionPassToMCFGPass g) CFG) fnid = None.
+Proof.
+  intros.
+  unfold find_function in *.
+  simpl.
+  apply find_map_mapped_none;
+  auto.
+Qed.
+
+
+Hint Resolve  (find_function_none).
+Hint Rewrite  (find_function_none).
+
+Lemma find_function_lifted_definition_pass:
+  forall (CFG: mcfg)
+    (fnid: function_id)
+    (g: CFGDefinitionPass)
+    (PRESERVES_DEFN_IDENT: preserves_ident_definition g),
+    find_function  ((liftCFGDefinitionPassToMCFGPass g) CFG) fnid =
+    option_map g (find_function CFG fnid).
+Proof.
+  intros.
+  remember (find_function CFG fnid) as FIND_F.
+  destruct FIND_F; simpl; auto.
+Qed.
+                                                        
+Hint Resolve(find_function_lifted_definition_pass).
+Hint Rewrite(find_function_lifted_definition_pass).
+
+
+Definition preserves_ident_block (g: BlockPass) : Prop :=
+  forall (b: block), blk_id (g b) = blk_id b.
+Hint Unfold preserves_ident_block.
+
+
+Lemma find_block: forall blks blkid (g: BlockPass) ,
+    preserves_ident_block g ->
+    find_block (map g blks) blkid = option_map  g (find_block blks blkid).
+Proof.
+  intros until g.
+  intros PRESERVES_IDENT.
+
+  induction blks.
+  - auto.
+  - simpl.
+    remember (blk_id a == blkid) as COND.
+
+    destruct COND.
+
+    + assert (BLKID_GA: blk_id (g a ) = blkid).
+      unfold preserves_ident_block in PRESERVES_IDENT.
+      rewrite <- e.
+      apply PRESERVES_IDENT.
+
+      destruct (blk_id (g a) == blkid); try contradiction; auto.
+
+    + assert (BLKID_GA: blk_id (g a ) <> blkid).
+      assert (BLK_ID_DEC: {blk_id (g a) = blkid} + {blk_id (g a) <> blkid}).
+      apply raw_id_eq_dec.
+      destruct BLK_ID_DEC; subst; try contradiction; auto.
+
+      destruct (blk_id (g a) == blkid); subst; try contradiction.
+      apply IHblks.
+Qed.
+
+Hint Resolve find_block.
+
+  
+(* If the pass preserves the terminator *)
+Definition preserves_block_terminator  (g: BlockPass): Prop :=
+  forall  (b: block), blk_term (g b) = blk_term b.
+
+
+Hint Unfold preserves_block_terminator.
+
+
+Lemma lifted_instr_pass_to_block_pass_preserves_block_terminator:
+  forall (pass: InstrPass),
+    preserves_block_terminator (liftInstrPassToBlockPass pass).
+Proof.
+  unfold preserves_block_terminator.
+  intros.
+  auto.
+Qed.
+Hint Resolve (lifted_instr_pass_to_block_pass_preserves_block_terminator).
+
+  
+
+Lemma rewrite_block_to_cmd_on_fetch_term: forall (g: block -> block) (b: block) pt,
+    blk_term_id b = pt -> 
+    preserves_block_terminator g ->
+    block_to_cmd (g b) pt = block_to_cmd b pt.
+Proof.
+  intros until  pt.
+  intros ACCESSING_TERMINATOR PRESERVES_TERMINATOR.
+  unfold preserves_block_terminator in PRESERVES_TERMINATOR.
+  
+  unfold block_to_cmd.
+  unfold blk_term_id.
+  rewrite PRESERVES_TERMINATOR.
+  subst.
+  unfold blk_term_id.
+
+  destruct (fst (blk_term b) == fst (blk_term b)); try contradiction.
+  auto.
+Qed.
+
+
+Hint Resolve (rewrite_block_to_cmd_on_fetch_term).
+
+Lemma rewrite_block_to_cmd_on_fetch_instr: forall (g: block -> block) (b: block) pt,
+    blk_term_id b <> pt -> 
+    preserves_block_terminator g ->
+    block_to_cmd (g b) pt = find_instr (blk_code (g b)) pt (fst (blk_term b)).
+Proof.
+  intros until  pt.
+  intros NOT_ACCESSING_TERMINATOR PRESERVES_TERMINATOR.
+  unfold preserves_block_terminator in PRESERVES_TERMINATOR.
+  
+  unfold block_to_cmd.
+  unfold blk_term_id in *.
+  rewrite PRESERVES_TERMINATOR.
+
+
+  destruct (fst (blk_term b) == pt); try contradiction.
+  auto.
+Qed.
+    
+Hint Resolve (rewrite_block_to_cmd_on_fetch_instr).
+
+
+
+Lemma preserves_types_implies_preserves_eval_expr: forall CFG g e t ex (pass: MCFGPass)
+  (PRESERVES_TYPES: preserves_types pass),
+  eval_exp (pass CFG) g e t ex =
+  eval_exp CFG g e t ex.
+Proof.
+  intros.
+  (* Use FunExt to make proof much shorter *)
+  assert (EVAL_TYP_EQ: eval_typ (pass CFG) = eval_typ CFG).
+  unfold eval_typ.
+  extensionality t0_ext.
+  unfold preserves_types in PRESERVES_TYPES.
+  rewrite PRESERVES_TYPES.
+  auto.
+  
+  intros.
+  unfold eval_exp.
+  rewrite EVAL_TYP_EQ.
+  reflexivity.
+Qed.
+
+Hint Resolve (preserves_types_implies_preserves_eval_expr).
+
+
+
+(* Jumps are defined with respect to the first instruction in the block.
+Create a definition that captures this notion *)
+Definition preserves_block_entry (pass: MCFGPass) : Prop :=
+  forall (MCFG: mcfg)
+    (fid: function_id)
+    (bid: block_id),
+    find_block_entry (pass MCFG) fid bid  = find_block_entry MCFG fid bid.
+
+Lemma lifted_instr_pass_to_MCFG_pass_preserves_block_entry:
+  forall (pass: InstrPass),
+    preserves_block_entry (liftCFGDefinitionPassToMCFGPass
+                             (liftCFGPassToCFGDefinitionPass
+                                (liftBlockPassToCFGPass
+                                   (liftInstrPassToBlockPass pass)))).
+Proof.
+  unfold preserves_block_entry.
+  intros.
+  unfold find_block_entry.
+  rewrite find_function_lifted_definition_pass; auto.
+  simpl.
+
+  destruct (find_function MCFG fid); auto.
+  simpl.
+
+
+  rewrite find_block; auto.
+  destruct (CFG.find_block (blks (df_instrs d)) bid); auto.
+
+  simpl.
+  unfold liftInstrPassToBlockPass.
+  unfold block_to_entry.
+  destruct b; simpl; auto.
+
+  repeat (destruct blk_code; simpl; auto).
+Qed.
+  
+  
+  
+
+  
+Lemma eq_jump: forall CFG fn  bk br g e s pass,
+    preserves_types pass ->
+    preserves_block_entry pass ->
+    jump (pass CFG) fn bk br g e s =
+    jump (CFG) fn bk br g e s.
+Proof.
+  intros until pass.
+  intros PRESRVES_TYPES.
+  intros PRESERVES_ENTRY.
+  unfold jump.
+
+  assert (EQ_EVAL_TYP: eval_typ (pass CFG) = eval_typ CFG).
+  unfold eval_typ.
+  extensionality typ.
+  apply preserves_types_implies_preserves_eval_typ; auto.
+  repeat (rewrite EQ_EVAL_TYP).
+
+  assert(EQ_EVAL_EXPR: eval_exp (pass CFG) = eval_exp (CFG)).
+  extensionality g_ext.
+  extensionality e_ext.
+  extensionality typ_ext.
+  extensionality expr_ext.
+  auto.
+
+  repeat(rewrite EQ_EVAL_EXPR).
+  
+  repeat (rewrite PRESERVES_ENTRY).
+  reflexivity.
+Qed.
+
+(* Helper function to run an InstrPass on the result of a find_instr. This
+is super kludgy.
+
+1. VE-LLVM's stuff is somewhat annoying to use, regarding the whole `cmd`.
+2. Coq could really use lenses :)
+*)
+Definition runInstrPassOnFindInstr
+           (pass: InstrPass)
+           (optin: option (cmd * option instr_id)) :
+  option (cmd * option instr_id) :=
+  let go (inp: cmd * option instr_id) :=
+      match inp with
+      | (Inst i, id) => (Inst (pass i), id)
+      | _ => inp
+      end
+  in option_map go optin.
+
+(* Characterise how find_instr behaves when we have an instruction pass.
+Since an instruction pass is not allowed to touch instruction IDs
+(this is the job of a `code` pass), intuitively, what we have is
+that we can find the instruction and then run the pass.
+
+This is slightly complicated by the fact that `find_instr` is used
+to find both instructions and terminators.
+
+Currently, our instruction pass does not allow modification of
+terminators. TODO, I guess...
+*)
+Lemma findOverInstrPassLiftedToIdInstrPass:
+  forall (pass: InstrPass)
+    (c: code)
+    (p: instr_id)
+    (termid: instr_id),
+    find_instr (map (liftInstrPassToIdInstrPass pass) c) p termid =
+    runInstrPassOnFindInstr pass (find_instr c p termid).
+Proof.
+  intros until c.
+  induction c; intros; unfold find_instr;
+    simpl; auto.
+
+  destruct a; simpl.
+  destruct (p == i); simpl.
+  - unfold liftInstrPassToIdInstrPass. unfold fallthrough.
+    destruct c; auto.
+
+  - fold find_instr. apply IHc.
+Qed.
+
+Hint Resolve findOverInstrPassLiftedToIdInstrPass.
+
+Lemma InstrPassPreservesBlockToCmd: forall (pass: InstrPass)
+                                      (b: block)
+                                      pt,
+    block_to_cmd ((liftInstrPassToBlockPass pass) b) pt  =
+    runInstrPassOnFindInstr pass (block_to_cmd b pt).
+Proof.
+  intros.
+  unfold block_to_cmd.
+  simpl.
+
+  assert (PRESERVES_TERM: blk_term ((liftInstrPassToBlockPass pass) b) =
+                          blk_term b).
+  auto.
+
+  unfold blk_term_id.
+  rewrite PRESERVES_TERM.
+
+  destruct (fst (blk_term b) == pt); auto.
+Qed.
+  
+
+Definition preserves_function_entry (pass: MCFGPass): Prop :=
+  forall (MCFG: mcfg) (fnid: function_id),
+    find_function_entry (pass MCFG) fnid = find_function_entry MCFG fnid.
+
+(* We need a  lifted instruction pass because the function entry
+is defined in terms of the entry of the first basic block. This is
+defined in terms of the ID OF THE FIRST INSTRUCTION.
+*)
+Lemma  lifted_instr_pass_preserves_function_entry:
+  forall (pass: InstrPass),
+    preserves_function_entry (liftCFGDefinitionPassToMCFGPass
+                                (liftCFGPassToCFGDefinitionPass
+                                   (liftBlockPassToCFGPass
+                                      (liftInstrPassToBlockPass pass)))) .
+Proof.
+  unfold preserves_function_entry.
+  intros.
+  unfold find_function_entry.
+  simpl.
+  rewrite find_function_lifted_definition_pass; auto.
+  destruct (find_function MCFG fnid); auto.
+
+  simpl.
+  rewrite find_block; auto.
+  destruct (CFG.find_block (blks (df_instrs d)) (init (df_instrs d))); auto.
+  simpl.
+
+  unfold blk_entry_id.
+  simpl.
+
+  destruct (blk_code b); simpl; auto.
+Qed.
+
+      
+  
+End PASSTHEOREMS.
+
+
+
+
+
+
