src/coq/StoreSwitch.v
@@ -1,0 +1,145 @@
+(* -------------------------------------------------------------------------- *
+ *                     Vellvm - the Verified LLVM project                     *
+ *                                                                            *
+ *     Copyright (c) 2017 Steve Zdancewic <stevez@cis.upenn.edu>              *
+ *                                                                            *
+ *   This file is distributed under the terms of the GNU General Public       *
+ *   License as published by the Free Software Foundation, either version     *
+ *   3 of the License, or (at your option) any later version.                 *
+ ---------------------------------------------------------------------------- *)
+
+Require Import ZArith List String Omega.
+Require Import Program.
+Require Import  Vellvm.Classes Vellvm.Util.
+Require Import Vellvm.LLVMAst.
+Require Import Vellvm.CFG.
+Require Import List ListDec.
+Require Import Vellvm.Pass.
+
+Import ListNotations.
+Open Scope Z_scope.
+Open Scope string_scope.
+
+Set Implicit Arguments.
+Set Contextual Implicit.
+
+Require Import Vellvm.Memory.
+
+
+Notation i32TY := (TYPE_I (32%Z)).
+Definition i32ARRTY := (TYPE_Array 2 i32TY).
+Definition i32ARRPTRTY := (TYPE_Pointer (TYPE_Array 2 i32TY)).
+Definition i32PTRTY := (TYPE_Pointer i32TY).
+Definition mkI32 (i: Z): texp := (i32TY, EXP_Integer i).
+
+(*
+
+Definition mkGEPI32 (name: string) (idx: Z) : texp :=
+  (xty, OP_GetElementPtr xty
+                   (xptrty, EXP_Ident (ID_Local (Name name)))
+                   ([mkI32 idx])).
+Definition mkXGEP := mkGEPI32.
+
+(* INSTR_Store (volatile:bool) (val:texp) (ptr:texp) (align:option int) *)
+Definition storeXAt0: instr_id * instr :=
+  (IVoid 0%Z, INSTR_Store false (mkI32 1) (mkXGEP "x" 0) None).
+
+Definition storeXAt1: instr_id * instr :=
+  (IVoid 1%Z, INSTR_Store false (mkI32 2) (mkXGEP "x" 1) None).
+*)
+
+(*
+
+        [(IId (Name "x"), INSTR_Alloca i32PTRTY (Some ((TYPE_I (32%Z)),  EXP_Integer 0)) None);
+           (IVoid 0%Z, INSTR_Store  false (TYPE_I (32%Z), EXP_Integer val1) p1 None);
+           (IVoid 1%Z, INSTR_Store  false (TYPE_I (32%Z), EXP_Integer val2) p2 None);
+           (IId (Name "xat0"), INSTR_Load false i32ty p3 None)]
+        ,
+        TERM_Ret (i32TY, (EXP_Ident (ID_Local (Name "xat0"))))
+      ) => None 
+ *)
+
+
+  (* (xty, OP_GetElementPtr xty
+                   (xptrty, EXP_Ident (ID_Local (Name name)))
+                   ([mkI32 idx])) *)
+
+Definition isGEPAtIx (e: texp) (ix: Z)  : bool :=
+  match e with
+  | ((TYPE_Array 2 i32TY),
+     OP_GetElementPtr (TYPE_Array 2 (TYPE_I 32%Z))
+                      (TYPE_Pointer (TYPE_Array 2 (TYPE_I 32%Z)),
+                       EXP_Ident (ID_Local (Name "x")))
+                      [(i32TY, EXP_Integer gepix)]) => if gepix =? ix
+                                                      then true
+                                                      else false
+  | (_, _) => false
+     end.
+                                                           
+
+                                 
+                                             
+Open Scope bool_scope.
+                                             
+Definition rewrite_main_bb (bb: block): option block := 
+  match blk_phis bb with
+  | [] => 
+    match (blk_code bb, blk_term bb) with
+    |  ([(IId (Name "x"), INSTR_Alloca i32PTRTY (Some ((TYPE_I (32%Z)),  EXP_Integer 0)) None) as i1;
+           (IVoid 0%Z, INSTR_Store  false (TYPE_I (32%Z), EXP_Integer 0) p1 None) as i2;
+           (IVoid 1%Z, INSTR_Store  false (TYPE_I (32%Z), EXP_Integer 1) p2 None) as i3;
+           (IId (Name "xat0"), INSTR_Load false (TYPE_I (32%Z)) p3 None) as i4] ,
+        (IVoid 2%Z, TERM_Ret (i32TY, (EXP_Ident (ID_Local (Name "xat0"))))) as iret) =>
+       if isGEPAtIx p1 0 && isGEPAtIx p2 1 && isGEPAtIx p3 0
+       then 
+         Some (mk_block (blk_id bb)
+                  (blk_phis bb)
+                  ([i1; i3; i2; i4])
+                   iret)
+       else None
+    | (_,_) => None
+    end
+      
+  | _ => None
+  end.
+
+Close Scope bool_scope.
+                                                      
+
+
+Definition rewrite_main_cfg (c: cfg) : cfg :=
+  {| init := init c;
+     blks := match blks c with
+             | [blk] => match rewrite_main_bb blk with
+                       | Some blk' => [blk']
+                       | None => [blk]
+                       end
+             | _ => blks c
+             end;
+     args := args c;
+|}.
+
+Definition rewrite_main_definition (d: definition cfg): definition cfg :=
+  if dc_name (df_prototype d) == (Name "main")
+  then
+    mk_definition cfg
+                  (df_prototype d) 
+                  (df_args d)
+                  (rewrite_main_cfg (df_instrs d))
+  else d.
+         
+
+  
+Definition rewrite_mcfg (MCFG:mcfg) : mcfg :=
+  {| m_name := m_name MCFG;
+     m_target:= m_target MCFG;
+     m_datalayout := m_datalayout MCFG;
+     m_type_defs := m_type_defs MCFG;
+     m_globals := m_globals MCFG;
+     m_declarations := m_declarations MCFG;
+     m_definitions := match (m_globals MCFG , m_declarations MCFG, m_definitions MCFG) with
+                      | ([], [], [defn]) => [rewrite_main_definition defn]
+                      | (_, _, _) => m_definitions MCFG
+                      end
+  |}.
+  
