src/coq/StoreSwitchManualProof.v
@@ -1,0 +1,459 @@
+Require Import ZArith List String Omega.
+Require Import Vellvm.AstLib Vellvm.LLVMAst.
+Require Import Vellvm.Classes.
+Require Import Vellvm.Util.
+Require Import Vellvm.CFG.
+Require Import Vellvm.LLVMIO.
+Require Import Vellvm.DynamicValues.
+Require Import Vellvm.StepSemantics.
+Require Import  Vellvm.Classes Vellvm.Util.
+Require Import Vellvm.LLVMAst.
+Require Import Vellvm.TypeUtil.
+Require Import Vellvm.Memory.
+Require Import Vellvm.Trace.
+Require Import Setoid Morphisms.
+Require Import Coq.Setoids.Setoid.
+Require Import SetoidClass.
+Require Import Coq.Classes.RelationClasses.
+Require Import Coq.Classes.Equivalence.
+Require Import Vellvm.StoreSwitch.
+Require Import Vellvm.TopLevel.
+Require FunctionalExtensionality.
+Require Import Eqdep_dec.
+Require Import Classical.
+Require Import Vellvm.Trace.
+Require Import FSets.FMapAVL.
+Require Import Integers.
+Require Coq.Structures.OrderedTypeEx.
+Require Import ZMicromega.
+Import IO.DV.
+Import Trace.MonadVerif.
+Require Nsatz.
+
+(** Enable SSReflect for better rewrite **)
+From mathcomp Require ssreflect ssrbool ssrfun bigop.
+Import ssreflect.SsrSyntax.
+Set Implicit Arguments.
+Unset Strict Implicit.
+Unset Printing Implicit Defensive.
+
+
+(** MEMORY **)          
+(** MEMORY **)          
+(** MEMORY **)          
+(** MEMORY **)          
+(** MEMORY **)          
+(** MEMORY **)          
+(** MEMORY **)          
+(** MEMORY **)          
+(** MEMORY **)          
+(** MEMORY **)          
+(** MEMORY **)          
+
+
+Check (M.memD).
+Check (M.memD M.empty).
+
+    
+
+(** PROGRAM **)
+(** PROGRAM **)
+(** PROGRAM **)
+(** PROGRAM **)
+(** PROGRAM **)
+(** PROGRAM **)
+(** PROGRAM **)
+(** PROGRAM **)
+(** PROGRAM **)
+(** PROGRAM **)
+(** PROGRAM **)
+  
+Open Scope Z_scope.
+Open Scope string_scope.
+Open Scope list_scope.
+
+Definition simpleProgramInitBBId : block_id := Name "entry".
+                                
+
+Notation i32ty := (TYPE_I (32%Z)).
+Notation i8ty := (TYPE_I (8%Z)).
+Notation i32ptrty :=  (TYPE_Pointer i32ty).
+Notation i8ptrty :=  (TYPE_Pointer i8ty).
+Definition mkI32 (i: Z): texp :=
+  (i32ty, EXP_Integer i).
+
+
+Definition mkI8 (i: Z): texp :=
+  (i8ty, EXP_Integer i).
+
+Definition xty := TYPE_Array 2 i32ty.
+Definition xptrty := TYPE_Pointer xty.
+Definition mkLLVMInt (i: Z): texp := mkI32 i.
+
+
+
+
+ (*INSTR_Alloca (t:typ) (nb: option texp) (align:option int)  *)
+Definition allocaX : instr_id * instr :=
+  (IId (Name "x"),
+   INSTR_Alloca (xptrty) (Some (mkLLVMInt 0)) None).
+
+Definition xexpr: texp := (xptrty, EXP_Ident (ID_Local (Name "x"))).
+
+(* OP_GetElementPtr    (t:typ) (ptrval:(typ * exp)) (idxs:list (typ * exp)) *)
+Definition mkGEPI32 (name: string) (idx: Z) : texp :=
+  (xty, OP_GetElementPtr xty
+                   (xptrty, EXP_Ident (ID_Local (Name name)))
+                   ([mkI32 idx])).
+
+
+Definition mkGEPI8 (name: string) (idx: Z) : texp :=
+  (i8ptrty, OP_GetElementPtr i8ty
+                   (i8ptrty, EXP_Ident (ID_Local (Name name)))
+                   ([mkI32 idx])).
+
+Definition mkXGEP := mkGEPI32.
+
+(* INSTR_Store (volatile:bool) (val:texp) (ptr:texp) (align:option int) *)
+Definition storeXAt0: instr_id * instr :=
+  (IVoid 0%Z, INSTR_Store false (mkLLVMInt 1) (mkXGEP "x" 0) None).
+
+Definition storeXAt1: instr_id * instr :=
+  (IVoid 1%Z, INSTR_Store false (mkLLVMInt 2) (mkXGEP "x" 1) None).
+
+(* INSTR_Load  (volatile:bool) (t:typ) (ptr:texp) (align:option int)  *)
+Definition loadXAt0: instr_id * instr :=
+  (IId (Name "xat0"), INSTR_Load false i32ty (mkXGEP "x" 0) None).
+  
+Definition pcfg : cfg := 
+{|
+  init := simpleProgramInitBBId;
+  blks := [{|
+      blk_id     := simpleProgramInitBBId;
+      blk_phis  := [];
+      blk_code  := [ allocaX; storeXAt0; storeXAt1; loadXAt0 ];
+      blk_term  := ((IVoid 2%Z),
+                    TERM_Ret (i32ty, (EXP_Ident (ID_Local (Name "xat0")))))
+    |}];
+  args := [];
+  |}.
+
+  
+Definition mainproto : declaration :=
+  {|
+    dc_name        := Name "main";
+    dc_type        :=  TYPE_Function TYPE_Void [TYPE_I 32];
+    dc_param_attrs := ([], []);
+    dc_linkage     := None;
+    dc_visibility  := None;
+    dc_dll_storage := None;
+    dc_cconv       := None;
+    dc_attrs       := [];
+    dc_section     := None;
+    dc_align       := None;
+    dc_gc          := None;
+
+  |}.
+
+
+Definition pmain : definition cfg  :=
+  {|
+    df_prototype   := mainproto;
+    df_args        := [];
+    df_instrs      := pcfg;
+  |}.
+
+Definition program : mcfg :=
+  {|
+    m_name := None;
+    m_target := None;
+    m_datalayout := None;
+    m_type_defs := [];
+    m_globals := [];
+    m_declarations := [];
+    m_definitions:= [pmain];
+  |}.
+
+
+(** Modified program **)
+
+  
+Definition pcfg' : cfg := 
+{|
+  init := simpleProgramInitBBId;
+  blks := [{|
+      blk_id     := simpleProgramInitBBId;
+      blk_phis  := [];
+      blk_code  := [ allocaX; storeXAt1; storeXAt0; loadXAt0 ];
+      blk_term  := ((IVoid 2%Z),
+                    TERM_Ret (i32ty, (EXP_Ident (ID_Local (Name "xat0")))))
+    |}];
+  args := [];
+|}.
+  
+Definition pmain' : definition cfg  :=
+  {|
+    df_prototype   := mainproto;
+    df_args        := [];
+    df_instrs      := pcfg';
+  |}.
+Definition program': mcfg := 
+  {|
+    m_name := None;
+    m_target := None;
+    m_datalayout := None;
+    m_type_defs := [];
+    m_globals := [];
+    m_declarations := [];
+    m_definitions:= [pmain'];
+  |}.
+Close Scope list_scope.
+
+
+
+Lemma program_program'_register_fn_eq:
+  TopLevel.SS.register_functions
+    program
+    (TopLevel.SS.ENV.empty IO.DV.dvalue) ≡
+    TopLevel.SS.register_functions
+    program'
+    (TopLevel.SS.ENV.empty IO.DV.dvalue) /\
+  TopLevel.SS.register_functions program
+                                 (TopLevel.SS.ENV.empty IO.DV.dvalue) =
+Trace.Tau
+    (TopLevel.SS.register_declaration (TopLevel.SS.ENV.empty IO.DV.dvalue)
+                                      mainproto).
+Proof.
+  
+  unfold TopLevel.SS.register_functions.
+  simpl.
+  split.
+  + rewrite bindM_Ret.
+    unfold TopLevel.SS.register_declaration.
+    simpl.
+    auto.
+
+  +  rewrite Trace.matchM. simpl.  auto.
+Qed.
+  
+  
+
+Lemma program_program'_build_global_environment_eq:
+   TopLevel.SS.build_global_environment program ≡
+                                        TopLevel.SS.build_global_environment program'.
+Proof.
+  unfold TopLevel.SS.build_global_environment.
+  simpl.
+
+  unfold TopLevel.SS.allocate_globals.
+  simpl.
+  
+  repeat (rewrite bindM_Ret).
+
+  destruct program_program'_register_fn_eq as [FN_EQ FN_VAL].
+
+  unfold TopLevel.SS.initialize_globals. simpl.
+  euttnorm.
+Qed.
+
+
+Lemma build_global_env_program_value:
+  TopLevel.SS.build_global_environment program ≡ Ret (TopLevel.SS.ENV.empty dvalue).
+Proof.
+  unfold TopLevel.SS.build_global_environment.
+  simpl.
+  unfold TopLevel.SS.allocate_globals.
+  simpl.
+  rewrite bindM_Ret.
+
+  
+  unfold TopLevel.SS.register_functions.
+  simpl.
+
+  assert ((bindM (Ret (TopLevel.SS.ENV.empty dvalue))
+       (fun y : TopLevel.SS.genv =>
+          TopLevel.SS.register_declaration y mainproto)) ≡
+                                                         (fun y => TopLevel.SS.register_declaration y mainproto) (TopLevel.SS.ENV.empty dvalue)).
+  rewrite bindM_Ret.
+  auto.
+Abort.
+
+Lemma eval_typ_i32: forall (CFG:mcfg), SS.eval_typ (CFG )i32ty = DTYPE_I 32.
+Proof.
+  intros.
+  unfold SS.eval_typ.
+  rewrite normalize_type_equation.
+  auto.
+Qed.
+
+
+Lemma eval_typ_i8: forall (CFG: mcfg), SS.eval_typ (CFG) i8ty = DTYPE_I 8.
+Proof.
+  intros.
+  unfold SS.eval_typ.
+  rewrite normalize_type_equation.
+  auto.
+Qed.
+
+Lemma eval_typ_array_i32: forall (CFG: mcfg),
+    (SS.eval_typ CFG (TYPE_Array 2 i32ty)) =
+    DTYPE_Array 2 (DTYPE_I 32).
+Proof.
+  intros.
+  unfold SS.eval_typ.
+  repeat (rewrite normalize_type_equation; simpl).
+  auto.
+Qed.
+
+Hint Resolve eval_typ_i32 : euttnormdb.
+Hint Resolve eval_typ_i8 : euttnormdb.
+Hint Resolve eval_typ_array_i32 : euttnormdb.
+Hint Rewrite eval_typ_i32 : euttnormdb.
+Hint Rewrite eval_typ_i8 : euttnormdb.
+Hint Rewrite eval_typ_array_i32 : euttnormdb.
+
+Hint Transparent SS.init_state.
+Hint Unfold SS.init_state.
+
+
+
+(** ALL HELL BREAKS LOOSE OTHERWISE **)
+Opaque M.add_all_index.
+Opaque M.lookup_all_index.
+         
+(** Show what the original program produces **)
+Open Scope list_scope.
+Theorem original_program_execution:
+   M.memD M.empty
+    (bindM (TopLevel.SS.init_state program "main")
+       (fun s : TopLevel.SS.state =>
+          TopLevel.SS.step_sem program (TopLevel.SS.Step s))) ≡
+    Ret (DVALUE_I32  (Int32.repr 1%Z)).
+Proof.
+  simpl.
+  unfold SS.init_state.
+  simpl.
+  unfold SS.build_global_environment.
+  simpl.
+  unfold SS.allocate_globals.
+  simpl.
+
+  euttnorm.
+  unfold SS.register_functions.
+  simpl.
+  euttnorm.
+  unfold SS.register_declaration.
+  euttnorm.
+  Set Ltac debug.
+  forcetrace.
+  euttnorm.
+  unfold SS.initialize_globals.
+
+    repeat (  euttnorm ||
+        M.forcememd ||
+        SS.forcestepsem ||
+        unfold SS.cont;simpl).
+
+    rewrite @Trace.matchM with (i := bindM _ _).
+    simpl.
+    euttnorm.
+    repeat (rewrite <- tauN_eutt_1).
+    simpl.
+    (* TODO: Why does the tactic rewrite not work?! WTF *)
+    (* rewrite force_memD_ret. *)
+    SS.forcestepsem.
+    simpl.
+    rewrite @Trace.matchM with (i := M.memD _ _).
+    simpl.
+    unfold xty.
+    simpl.
+    replace (Int32.unsigned (Int32.repr 0)) with 0.
+    replace (Int32.unsigned (Int32.repr 1)) with 1.
+    simpl.
+    rewrite (M.lookup_all_index_of_add_all_index_no_alias).
+    rewrite (M.lookup_all_index_of_add_all_index_full_alias).
+    unfold M.sbyte_list_to_Z.
+    simpl.
+    simpl.
+    simpl.
+    auto.
+    auto.
+    simpl.
+    omega.
+    rewrite Int.unsigned_repr; try omega; auto.
+    unfold Int.max_unsigned.
+    unfold Int.modulus.
+    simpl.
+    omega.
+    rewrite Int.unsigned_repr; try omega; auto.
+    unfold Int.max_unsigned.
+    unfold Int.modulus.
+    simpl.
+    omega.
+Qed.
+
+    
+Close Scope list_scope.
+
+
+
+Theorem new_program_execution:
+   M.memD M.empty
+    (bindM (TopLevel.SS.init_state program' "main")
+       (fun s : TopLevel.SS.state =>
+          TopLevel.SS.step_sem program' (TopLevel.SS.Step s))) ≡
+    Ret (DVALUE_I32 (Int32.repr 1%Z)).
+Proof.
+  simpl.
+  unfold SS.init_state.
+  simpl.
+  unfold SS.build_global_environment.
+  simpl.
+  unfold SS.allocate_globals.
+  simpl.
+
+  euttnorm.
+  unfold SS.register_functions.
+  simpl.
+  euttnorm.
+  unfold SS.register_declaration.
+  euttnorm.
+  forcetrace.
+  euttnorm.
+  unfold SS.initialize_globals.
+
+    repeat (  euttnorm ||
+        M.forcememd ||
+        SS.forcestepsem ||
+        unfold SS.cont;simpl).
+
+    rewrite @Trace.matchM with (i := bindM _ _).
+    simpl.
+    euttnorm.
+    repeat (rewrite <- tauN_eutt_1).
+    simpl.
+    (* TODO: Why does the tactic rewrite not work?! WTF *)
+    (* rewrite force_memD_ret. *)
+    SS.forcestepsem.
+    simpl.
+    rewrite @Trace.matchM with (i := M.memD _ _).
+    simpl.
+    unfold xty.
+    simpl.
+    replace (Int32.unsigned (Int32.repr 0)) with 0; auto.
+    replace (Int32.unsigned (Int32.repr 1)) with 1; auto.
+    simpl.
+    rewrite M.lookup_all_index_of_add_all_index_full_alias; auto.
+    
+Qed.
+
+(** State what we want to prove **)
+Definition program_program'_have_same_semantics:
+    run_mcfg_with_memory program ≡ run_mcfg_with_memory program'.
+Proof.
+  unfold run_mcfg_with_memory.
+  rewrite original_program_execution.
+  rewrite new_program_execution.
+  reflexivity.
+Qed.
+      
