src/coq/StoreSwitchProof.v
@@ -1,0 +1,389 @@
+
+(* -------------------------------------------------------------------------- *
+ *                     Vellvm - the Verified LLVM project                     *
+ *                                                                            *
+ *     Copyright (c) 2017 Steve Zdancewic <stevez@cis.upenn.edu>              *
+ *                                                                            *
+ *   This file is distributed under the terms of the GNU General Public       *
+ *   License as published by the Free Software Foundation, either version     *
+ *   3 of the License, or (at your option) any later version.                 *
+ ---------------------------------------------------------------------------- *)
+
+
+Require Import ZArith List String Omega.
+Require Import Vellvm.AstLib Vellvm.LLVMAst.
+Require Import Vellvm.Classes.
+Require Import Vellvm.Util.
+Require Import Vellvm.CFG.
+Require Import Vellvm.LLVMIO.
+Require Import Vellvm.DynamicValues.
+Require Import  Vellvm.Classes Vellvm.Util.
+Require Import Vellvm.LLVMAst.
+Require Import Vellvm.TypeUtil.
+Require Import Vellvm.Memory.
+Require Import Vellvm.Trace.
+Require Import Setoid Morphisms.
+Require Import Coq.Setoids.Setoid.
+Require Import SetoidClass.
+Require Import Coq.Classes.RelationClasses.
+Require Import Coq.Classes.Equivalence.
+Require Import Vellvm.StoreSwitch.
+Require Import Vellvm.TopLevel.
+Require FunctionalExtensionality.
+Require Import Eqdep_dec.
+Require Import Classical.
+Import Trace.MonadVerif.
+
+
+From mathcomp Require ssreflect ssrbool ssrfun bigop.
+Import ssreflect.SsrSyntax.
+Set Implicit Arguments.
+Unset Strict Implicit.
+Unset Printing Implicit Defensive.
+
+
+Open Scope Z_scope.
+Open Scope string_scope.
+
+
+
+
+Module STORESWITCHPROOF (A:MemoryAddress.ADDRESS) (LLVMIO:LLVM_INTERACTIONS(A)).
+  (* Need this to simplify proofs, otherwise I need to painfully destruct
+  execution chains. *)
+Import FunctionalExtensionality.
+
+Import SS.
+Import LLVMIO.
+
+Lemma bindM_Raise: forall {X Y : Type} (e : string) (f: X -> M IO Y),
+    bindM (raise e) f ≡ raise e.
+Proof.
+  intros.
+  unfold raise.
+  unfold exn_trace.
+  euttnorm.
+Qed.
+Hint Rewrite (@bindM_Raise) : euttnormdb.
+    
+
+Lemma  eval_type_I64: forall (cfg: mcfg),
+    eval_typ cfg (TYPE_I 64) = DTYPE_I 64.
+Proof.
+  intros.
+  unfold eval_typ.
+  rewrite normalize_type_equation.
+  auto.
+Qed.
+
+
+Hint Resolve eval_type_I64.
+
+Lemma eval_typ_equals: forall (mcfg: mcfg) (t: typ),
+    eval_typ (rewrite_mcfg mcfg) t = eval_typ mcfg t.
+Proof.
+  intros.
+  repeat (unfold eval_typ).
+  repeat (rewrite normalize_type_equation).
+
+  destruct t; auto.
+Qed.
+
+Hint Resolve eval_typ_equals.
+Hint Rewrite eval_typ_equals.
+
+Definition patternMkGEPAtIx (ix: Z)  : texp :=
+  ((TYPE_Array 2 i32TY), OP_GetElementPtr (TYPE_Array 2 (TYPE_I 32%Z))
+                                          (TYPE_Pointer (TYPE_Array 2 (TYPE_I 32%Z)),
+                                           EXP_Ident (ID_Local (Name "x")))
+                                          [(i32TY, EXP_Integer ix)]).
+
+Definition codeToMatch  : code :=
+     [(IId (Name "x"), INSTR_Alloca i32PTRTY (Some ((TYPE_I (32%Z)),  EXP_Integer 0)) None);
+        (IVoid 0%Z, INSTR_Store  false (TYPE_I (32%Z), EXP_Integer 0)
+                                 (patternMkGEPAtIx 0) None);
+        (IVoid 1%Z, INSTR_Store  false (TYPE_I (32%Z), EXP_Integer 1) (patternMkGEPAtIx 1) None);
+        (IId (Name "xat0"), INSTR_Load false (TYPE_I (32%Z)) (patternMkGEPAtIx 0) None)].
+
+
+Lemma no_code_match_pattern_implies_no_rewrite:
+  forall (c: code)
+    (NOMATCH: c <> codeToMatch)
+    (bb: block)
+    (C_IS_CODE_BB: blk_code bb = c),
+    rewrite_main_bb  bb = None.
+Proof.
+  intros.
+  destruct bb; subst.
+  unfold rewrite_main_bb.
+  simpl.
+  destruct (blk_phis); try reflexivity.
+  destruct (blk_code); try reflexivity.
+  destruct p; try reflexivity.
+Admitted.
+
+Definition termToMatch : instr_id * terminator :=
+  (IVoid 2%Z, TERM_Ret (i32TY, (EXP_Ident (ID_Local (Name "xat0"))))).
+
+Lemma no_term_match_pattern_implies_no_rewrite:
+  forall (t: instr_id *terminator)
+    (NOMATCH: t <> termToMatch)
+    (bb: block)
+    (C_IS_CODE_BB: blk_term bb = t),
+    rewrite_main_bb  bb = None.
+Proof.
+  intros.
+  unfold rewrite_main_bb.
+Admitted.
+  
+
+Lemma m_globals_equals: forall (CFG: mcfg),
+    m_globals (rewrite_mcfg CFG) = m_globals CFG.
+Proof.
+  intros.
+  destruct CFG.
+  reflexivity.
+Qed.
+
+Hint Resolve m_globals_equals.
+Hint Rewrite m_globals_equals.
+
+Lemma m_declaration_equals: forall (CFG: mcfg),
+    m_declarations (rewrite_mcfg CFG)  = m_declarations CFG.
+Proof.
+  intros.
+  destruct CFG.
+  reflexivity.
+Qed.
+
+Hint Resolve m_declaration_equals.
+Hint Rewrite m_declaration_equals.
+
+Lemma preserves_prototypes: forall (CFG: mcfg),
+    map df_prototype (m_definitions (rewrite_mcfg CFG)) = map df_prototype (m_definitions CFG).
+Proof.
+  intros.
+  destruct CFG.
+  simpl.
+  destruct m_globals; try reflexivity.
+  destruct m_declarations; try reflexivity.
+  destruct m_definitions; try reflexivity.
+  destruct m_definitions; try reflexivity.
+  unfold rewrite_main_definition.
+  simpl.
+  destruct (dc_name (df_prototype d) == Name "main"); try reflexivity.
+Qed.
+
+
+
+Hint Resolve m_declaration_equals.
+Hint Rewrite m_declaration_equals.
+
+Lemma allocate_globals_equals: forall (CFG: mcfg),
+    TopLevel.SS.allocate_globals (rewrite_mcfg CFG) (m_globals (rewrite_mcfg CFG)) =
+    TopLevel.SS.allocate_globals CFG (m_globals CFG).
+Proof.
+  intros.
+  unfold TopLevel.SS.allocate_globals.
+  rewrite m_globals_equals.
+  destruct (m_globals CFG); try reflexivity.
+Qed.
+
+
+Hint Resolve allocate_globals_equals.
+Hint Rewrite allocate_globals_equals.
+
+Lemma find_function_entry_equals: forall (CFG: mcfg),
+    find_function_entry (rewrite_mcfg CFG) (Name "main") =
+    find_function_entry CFG (Name "main").
+Proof.
+  intros.
+Abort.
+
+Lemma register_functions_equal: forall (CFG: mcfg) (ge: TopLevel.SS.genv),
+    TopLevel.SS.register_functions (rewrite_mcfg CFG) ge ≡
+    TopLevel.SS.register_functions (CFG) ge.
+Proof.
+  intros.
+  unfold TopLevel.SS.register_functions.
+  simpl.
+  destruct m_globals; try reflexivity.
+  destruct m_declarations; try reflexivity.
+  destruct m_definitions; try reflexivity.
+  simpl.
+  destruct l; try reflexivity.
+  simpl.
+  intros.
+  euttnorm.
+  destruct d. simpl. unfold rewrite_main_definition. simpl.
+  destruct (dc_name df_prototype == Name "main"); try reflexivity.
+Qed.
+
+
+Hint Resolve register_functions_equal.
+Hint Rewrite register_functions_equal.
+
+Lemma ident_of_prototype_equal: forall (d: definition cfg),
+    ident_of (df_prototype (rewrite_main_definition d)) =
+    ident_of (df_prototype d).
+Proof.
+  intros.
+  destruct d. unfold rewrite_main_definition. simpl.
+  destruct (dc_name df_prototype == Name "main"); try reflexivity.
+Qed.
+
+                                   
+
+Hint Resolve ident_of_prototype_equal.
+Hint Rewrite ident_of_prototype_equal.
+
+Lemma find_block_of_rewritten_defn: forall (CFG: mcfg)
+                                  (GLOBALS_EMPTY: m_globals CFG = [])
+                                  (DECLARATIONS_EMPTY : m_declarations CFG = [])
+                                  (d : definition cfg)
+                                  (DEFINITIONS_VALUE : m_definitions CFG = [d])
+                                  (D_IS_MAIN : ident_of (df_prototype d) = ID_Global (Name "main")),
+    find_block (blks (df_instrs (rewrite_main_definition d)))
+               (init (df_instrs (rewrite_main_definition d))) =
+    find_block (blks (df_instrs (d)))
+               (init (df_instrs (d))).
+Proof.
+  intros.
+  unfold find_block.
+  unfold rewrite_main_definition.
+  simpl.
+  destruct (dc_name (df_prototype d) == Name "main"); try contradiction.
+  simpl.
+Abort.
+    
+            
+
+Theorem preserves_semantics:
+  forall (CFG: mcfg),
+    (run_mcfg_with_memory (rewrite_mcfg CFG)) ≡ (run_mcfg_with_memory CFG).
+Proof.
+  intros.
+  unfold run_mcfg_with_memory.
+  unfold TopLevel.SS.init_state.
+  unfold TopLevel.SS.build_global_environment.
+  rewrite m_globals_equals.
+  rewrite allocate_globals_equals.
+  (** Discard one choice of globals since we do nothing **)
+  destruct (m_globals CFG) eqn:globals;  try (unfold rewrite_mcfg; destruct CFG; simpl in *; rewrite globals; reflexivity).
+  simpl.
+  euttnorm.
+  unfold TopLevel.SS.allocate_globals; simpl.
+  euttnorm.
+
+  rewrite register_functions_equal.
+  unfold TopLevel.SS.register_functions.
+  simpl.
+
+  (** Show for both choices of declarations *)
+  destruct (m_declarations CFG) eqn:declarations;
+    try (unfold rewrite_mcfg; simpl in *; rewrite globals, declarations; simpl; reflexivity).
+
+  simpl.
+  (** Discard the case where definitions is empty **)
+  destruct (m_definitions CFG) eqn:definitions;
+    try (unfold rewrite_mcfg; destruct CFG; simpl in *; rewrite globals, declarations, definitions; simpl; reflexivity).
+
+  
+  (** Discard the case where definitions is too large **)
+  destruct l;
+    try (unfold rewrite_mcfg; destruct CFG; simpl in *; rewrite globals, declarations, definitions; simpl; reflexivity).
+
+  simpl.
+  euttnorm.
+  unfold register_declaration.
+  euttnorm.
+
+  repeat M.forcememd.
+  repeat euttnorm.
+
+  unfold initialize_globals; simpl.
+  repeat euttnorm.
+
+  
+  destruct (dc_name (df_prototype d) == Name "main").
+  + (** main function **)
+    assert (find_function_entry (rewrite_mcfg CFG) (Name "main") =
+            find_function_entry CFG (Name "main")).
+
+  (* find function entry *)
+  unfold find_function_entry.
+  simpl.
+
+  unfold find_function.
+  simpl.
+
+  unfold find_defn.
+  simpl.
+
+  rewrite globals, declarations, definitions.
+  simpl.
+
+  destruct (ident_of ((rewrite_main_definition d)) ==
+            ID_Global (Name "main")) as [DEF_REWRITE_MAIN | DEF_REWRITE_NOT_MAIN].
+  destruct (ident_of   d == ID_Global (Name "main")) as [DEF_MAIN | DEF_NOT_MAIN].
+
+  + (* We have both mains, the case we care about *)
+
+    
+    intros.
+    unfold find_block.
+    intros.
+    unfold rewrite_main_definition.
+    destruct (dc_name (df_prototype d) == Name "main") as [_ | CONTRA]; try contradiction.
+    simpl.
+    destruct (blks (df_instrs d)) eqn:BLKS; try auto.
+    destruct l; auto.
+
+
+    assert (CODE_MATCHES_DECIDABLE: {blk_code b = codeToMatch} + {blk_code b <> codeToMatch}).
+    apply code_eq_dec.
+    destruct CODE_MATCHES_DECIDABLE as [CODE_MATCHES  | CODE_DOES_NOT_MATCH];
+      try (erewrite no_code_match_pattern_implies_no_rewrite; eauto; fail).
+
+    
+    assert (TERM_MATCHES_DECIDABLE: {blk_term b = termToMatch} + {blk_term b <> termToMatch}).
+    decide equality; auto.
+    apply terminator_eq_dec.
+    destruct TERM_MATCHES_DECIDABLE as [TERM_MATCHES  | TERM_DOES_NOT_MATCH];
+      try (erewrite no_term_match_pattern_implies_no_rewrite; eauto; fail).
+
+
+
+              
+
+      unfold rewrite_main_definition. simpl.
+      assert (DEF_NAME_MAIN': dc_name (df_prototype d) = Name "main").
+      simpl.
+      unfold ident_of in DEF_MAIN.
+      unfold ident_of_declaration in DEF_MAIN.
+      inversion DEF_MAIN.
+      auto.
+      
+      destruct (dc_name (df_prototype d) == Name "main"); try contradiction.
+    * admit.
+    * admit.
+      
+    
+  + (** not main **)
+    destruct (ident_of (df_prototype (rewrite_main_definition d)) ==
+              ID_Global (Name "main")) as [DEF_REWRITE_MAIN | DEF_REWRITE_NOT_MAIN].
+    * (** rewrite has main, this is contradiction since we do not change names *)
+      cut (ident_of (df_prototype d) = ident_of (df_prototype (rewrite_main_definition d)));
+        try apply preserves_prototypes; auto.
+      intros IDENT_EQUAL.
+      rewrite IDENT_EQUAL, DEF_REWRITE_MAIN in DEF_NOT_MAIN.
+      contradiction.
+      simpl.
+      euttnorm.
+      unfold raise.
+      unfold IO.exn_trace.
+      euttnorm.
+Abort.
+  
+
+End STORESWITCHPROOF.
